added submission

thys/IMAP-CRDT/IMAP-proof-helpers.thy
@@ -1,12 +1,15 @@
 section {* Proof Helpers *}
 
+text\<open>In this section we define and prove lemmas that help to show that all identified critical conditions hold for concurrent operations.
+Many of the following parts are derivations from the definitions and lemmas of Gomes et al.\<close>
+
 theory
   "IMAP-proof-helpers"
 imports
-  "IMAP-def"	
+  "IMAP-def"  
 
 begin
-	
+  
 lemma (in imap) apply_operations_never_fails:
   assumes "xs prefix of i"
   shows "apply_operations xs \<noteq> None"
@@ -22,17 +25,17 @@ using assms proof(induction xs rule: rev_induct, clarsimp)
   qed
 qed
 
-lemma (in imap) add_id_valid:
+lemma (in imap) create_id_valid:
   assumes "xs prefix of j"
-    and "Deliver (i1, Add i2 e) \<in> set xs"
+    and "Deliver (i1, Create i2 e) \<in> set xs"
   shows "i1 = i2"
 proof -
-  have "\<exists>s. valid_behaviours s (i1, Add i2 e)"
+  have "\<exists>s. valid_behaviours s (i1, Create i2 e)"
     using assms deliver_in_prefix_is_valid by blast
   thus ?thesis
     by(simp add: valid_behaviours_def)
 qed
-	
+  
 lemma (in imap) append_id_valid:
   assumes "xs prefix of j"
     and "Deliver (i1, Append i2 e) \<in> set xs"
@@ -43,7 +46,7 @@ proof -
   thus ?thesis
     by(simp add: valid_behaviours_def)
 qed
-	
+  
 lemma (in imap) expunge_id_valid:
   assumes "xs prefix of j"
     and "Deliver (i1, Expunge e mo i2) \<in> set xs"
@@ -54,7 +57,7 @@ proof -
   thus ?thesis
     by(simp add: valid_behaviours_def)
 qed
-	
+  
 lemma (in imap) store_id_valid:
   assumes "xs prefix of j"
     and "Deliver (i1, Store e mo i2) \<in> set xs"
@@ -68,22 +71,22 @@ qed
 
 definition (in imap) added_ids :: "('id \<times> ('id, 'b) operation) event list \<Rightarrow> 'b \<Rightarrow> 'id list" where
   "added_ids es p \<equiv> List.map_filter (\<lambda>x. case x of 
-		Deliver (i, Add j e) \<Rightarrow> if e = p then Some j else None | 
+    Deliver (i, Create j e) \<Rightarrow> if e = p then Some j else None | 
     Deliver (i, Expunge e mo j) \<Rightarrow> if e = p then Some j else None |
-		_ \<Rightarrow> None) es"
-	
+    _ \<Rightarrow> None) es"
+  
 definition (in imap) added_files :: "('id \<times> ('id, 'b) operation) event list \<Rightarrow> 'b \<Rightarrow> 'id list" where
     "added_files es p \<equiv> List.map_filter (\<lambda>x. case x of 
-		Deliver (i, Append j e) \<Rightarrow> if e = p then Some j else None |
+    Deliver (i, Append j e) \<Rightarrow> if e = p then Some j else None |
     Deliver (i, Store e mo j) \<Rightarrow> if e = p then Some j else None |
-		_ \<Rightarrow> None) es"
-		
+    _ \<Rightarrow> None) es"
+    
 -- {* added files simplifier *}
   
 lemma (in imap) [simp]:
   shows "added_files [] e = []"
   by (auto simp: added_files_def map_filter_def)
-  	
+    
 lemma (in imap) [simp]:
   shows "added_files (xs @ ys) e = added_files xs e @ added_files ys e"
     by (auto simp: added_files_def map_filter_append)
@@ -92,12 +95,12 @@ lemma (in imap) added_files_Broadcast_collapse [simp]:
   shows "added_files ([Broadcast e]) e' = []"
   by (auto simp: added_files_def map_filter_append map_filter_def)
     
-lemma (in imap) added_files_Deliver_Rem_collapse [simp]:
-  shows "added_files ([Deliver (i, Rem is e)]) e' = []"
+lemma (in imap) added_files_Deliver_Delete_collapse [simp]:
+  shows "added_files ([Deliver (i, Delete is e)]) e' = []"
   by (auto simp: added_files_def map_filter_append map_filter_def)
     
-lemma (in imap) added_files_Deliver_Add_collapse [simp]:
-  shows "added_files ([Deliver (i, Add j e)]) e' = []"
+lemma (in imap) added_files_Deliver_Create_collapse [simp]:
+  shows "added_files ([Deliver (i, Create j e)]) e' = []"
   by (auto simp: added_files_def map_filter_append map_filter_def)
 
 lemma (in imap) added_files_Deliver_Expunge_collapse [simp]:
@@ -111,7 +114,7 @@ lemma (in imap) added_files_Deliver_Append_diff_collapse [simp]:
 lemma (in imap) added_files_Deliver_Append_same_collapse [simp]:
   shows "added_files ([Deliver (i, Append j e)]) e = [j]"
   by (auto simp: added_files_def map_filter_append map_filter_def)
-  	
+    
 lemma (in imap) added_files_Deliver_Store_diff_collapse [simp]:
   shows "e \<noteq> e' \<Longrightarrow> added_files ([Deliver (i, Store e mo j)]) e' = []"
   by (auto simp: added_files_def map_filter_append map_filter_def)
@@ -119,14 +122,14 @@ lemma (in imap) added_files_Deliver_Store_diff_collapse [simp]:
 lemma (in imap) added_files_Deliver_Store_same_collapse [simp]:
   shows "added_files ([Deliver (i, Store e mo j)]) e = [j]"
   by (auto simp: added_files_def map_filter_append map_filter_def)
-  	
+    
  
 -- {* added ids simplifier *}
   
 lemma (in imap) [simp]:
   shows "added_ids [] e = []"
   by (auto simp: added_ids_def map_filter_def)
-  	
+    
 lemma (in imap) split_ids [simp]:
   shows "added_ids (xs @ ys) e = added_ids xs e @ added_ids ys e"
     by (auto simp: added_ids_def map_filter_append)
@@ -135,34 +138,34 @@ lemma (in imap) added_ids_Broadcast_collapse [simp]:
   shows "added_ids ([Broadcast e]) e' = []"
   by (auto simp: added_ids_def map_filter_append map_filter_def)
     
-lemma (in imap) added_ids_Deliver_Rem_collapse [simp]:
-  shows "added_ids ([Deliver (i, Rem is e)]) e' = []"
+lemma (in imap) added_ids_Deliver_Delete_collapse [simp]:
+  shows "added_ids ([Deliver (i, Delete is e)]) e' = []"
   by (auto simp: added_ids_def map_filter_append map_filter_def)
     
 lemma (in imap) added_ids_Deliver_Append_collapse [simp]:
   shows "added_ids ([Deliver (i, Append j e)]) e' = []"
   by (auto simp: added_ids_def map_filter_append map_filter_def)
-  	
+    
 lemma (in imap) added_ids_Deliver_Store_collapse [simp]:
   shows "added_ids ([Deliver (i, Store e mo j)]) e' = []"
   by (auto simp: added_ids_def map_filter_append map_filter_def)
     
-lemma (in imap) added_ids_Deliver_Add_diff_collapse [simp]:
-  shows "e \<noteq> e' \<Longrightarrow> added_ids ([Deliver (i, Add j e)]) e' = []"
+lemma (in imap) added_ids_Deliver_Create_diff_collapse [simp]:
+  shows "e \<noteq> e' \<Longrightarrow> added_ids ([Deliver (i, Create j e)]) e' = []"
   by (auto simp: added_ids_def map_filter_append map_filter_def)
-  	
+    
 lemma (in imap) added_ids_Deliver_Expunge_diff_collapse [simp]:
   shows "e \<noteq> e' \<Longrightarrow> added_ids ([Deliver (i, Expunge e mo j)]) e' = []"
   by (auto simp: added_ids_def map_filter_append map_filter_def)
     
-lemma (in imap) added_ids_Deliver_Add_same_collapse [simp]:
-  shows "added_ids ([Deliver (i, Add j e)]) e = [j]"
+lemma (in imap) added_ids_Deliver_Create_same_collapse [simp]:
+  shows "added_ids ([Deliver (i, Create j e)]) e = [j]"
   by (auto simp: added_ids_def map_filter_append map_filter_def)
-  	
+    
 lemma (in imap) added_ids_Deliver_Expunge_same_collapse [simp]:
   shows "added_ids ([Deliver (i, Expunge e mo j)]) e = [j]"
   by (auto simp: added_ids_def map_filter_append map_filter_def)
-  	
+    
 lemma (in imap) expunge_id_not_in_set:
   assumes "i1 \<notin> set (added_ids [Deliver (i, Expunge e mo i2)] e)"
   shows "i1 \<noteq> i2"
@@ -208,15 +211,16 @@ using assms proof (induct xs rule: rev_induct, clarsimp)
     case X: (Deliver e')
     moreover obtain a b where E: "e' = (a, b)" by force
     ultimately show ?thesis
-      using snoc apply (case_tac b; clarify)
-       apply (simp,metis prefix_of_appendD)
-        apply force using  append_id_valid
-        apply simp using E 
-      apply (metis added_files_Deliver_Append_diff_collapse added_files_Deliver_Append_same_collapse empty_iff in_set_conv_decomp list.set(1) prefix_of_appendD set_ConsD)
-      	apply simp using E apply_operations_added_files
-      apply blast apply simp using E apply_operations_added_files 
+      using snoc apply (case_tac b; clarify) apply (simp,metis prefix_of_appendD)
+        apply force 
+      using append_id_valid apply simp 
+      using E apply (metis added_files_Deliver_Append_diff_collapse added_files_Deliver_Append_same_collapse empty_iff in_set_conv_decomp list.set(1) prefix_of_appendD set_ConsD)
+        apply simp 
+      using E apply_operations_added_files apply blast 
+        apply simp 
+      using E apply_operations_added_files 
       by (metis Un_iff added_files_Deliver_Store_diff_collapse added_files_Deliver_Store_same_collapse empty_iff empty_set list.set_intros(1) prefix_of_appendD set_ConsD set_append store_id_valid)
   qed
 qed
-	
+  
 end
