thys/IMAP-CRDT/IMAP-proof-independent.thy
@@ -1,15 +1,18 @@
 section {* Independence of IMAP Commands *}
 
+text\<open>In this section we show that two concurrent operations that reference to the same tag must be identical.\<close>
+
 theory
   "IMAP-proof-independent"
 imports
   "IMAP-def"
-  "IMAP-proof-helpers"	
+  "IMAP-proof-helpers"  
 begin
   
 lemma (in imap) Broadcast_Expunge_Deliver_prefix_closed:
   assumes "xs @ [Broadcast (i, Expunge e mo i)] prefix of j"
-  shows "Deliver (mo, Append mo e) \<in> set xs \<or> (\<exists> mo2 . Deliver (mo, Store e mo2 mo) \<in> set xs)"
+  shows "Deliver (mo, Append mo e) \<in> set xs \<or> 
+    (\<exists> mo2 . Deliver (mo, Store e mo2 mo) \<in> set xs)"
 proof -  
   obtain y where "apply_operations xs = Some y"
     using assms broadcast_only_valid_msgs by blast
@@ -18,10 +21,11 @@ proof -
   ultimately show ?thesis
     using assms Deliver_added_files apply_operations_added_files by blast
 qed
-	
+  
 lemma (in imap) Broadcast_Store_Deliver_prefix_closed:
   assumes "xs @ [Broadcast (i, Store e mo i)] prefix of j"
-  shows "Deliver (mo, Append mo e) \<in> set xs \<or> (\<exists> mo2 . Deliver (mo, Store e mo2 mo) \<in> set xs)"
+  shows "Deliver (mo, Append mo e) \<in> set xs \<or> 
+    (\<exists> mo2 . Deliver (mo, Store e mo2 mo) \<in> set xs)"
 proof -  
   obtain y where "apply_operations xs = Some y"
     using assms broadcast_only_valid_msgs by blast
@@ -34,7 +38,8 @@ qed
 lemma (in imap) Deliver_added_ids:
   assumes "xs prefix of j"
     and "i \<in> set (added_ids xs e)"
-  shows "Deliver (i, Add i e) \<in> set xs \<or> (\<exists> mo . Deliver (i, Expunge e mo i) \<in> set xs)"
+  shows "Deliver (i, Create i e) \<in> set xs \<or> 
+    (\<exists> mo . Deliver (i, Expunge e mo i) \<in> set xs)"
 using assms proof (induct xs rule: rev_induct, clarsimp)
   case (snoc x xs) thus ?case
   proof (cases x, force)
@@ -42,22 +47,23 @@ using assms proof (induct xs rule: rev_induct, clarsimp)
     moreover obtain a b where "e' = (a, b)" by force
     ultimately show ?thesis
       using snoc apply (case_tac b; clarify)
-       apply (simp,metis added_ids_Deliver_Add_diff_collapse added_ids_Deliver_Add_same_collapse
-              empty_iff list.set(1) set_ConsD add_id_valid in_set_conv_decomp prefix_of_appendD)
-       apply force using  append_id_valid 
-      	
-       apply (simp, metis (no_types, lifting)  prefix_of_appendD)
-      
-      apply (simp)
-       apply (metis Un_iff added_ids_Deliver_Expunge_diff_collapse added_ids_Deliver_Expunge_same_collapse empty_iff expunge_id_valid list.set(1) list.set_intros(1) prefix_of_appendD set_ConsD set_append)
-        by (simp, blast)
+      apply (simp,metis added_ids_Deliver_Create_diff_collapse added_ids_Deliver_Create_same_collapse
+              empty_iff list.set(1) set_ConsD create_id_valid in_set_conv_decomp prefix_of_appendD)
+        apply force using  append_id_valid         
+          apply (simp, metis (no_types, lifting)  prefix_of_appendD)      
+            apply (simp)
+              apply (metis Un_iff added_ids_Deliver_Expunge_diff_collapse added_ids_Deliver_Expunge_same_collapse empty_iff expunge_id_valid list.set(1) list.set_intros(1) prefix_of_appendD set_ConsD set_append)
+      by (simp, blast)
   qed
 qed
 
 lemma (in imap) Broadcast_Deliver_prefix_closed:
-  assumes "xs @ [Broadcast (r, Rem ix e)] prefix of j"
+  assumes "xs @ [Broadcast (r, Delete ix e)] prefix of j"
     and "i \<in> ix"
-  shows "Deliver (i, Add i e) \<in> set xs \<or> Deliver (i, Append i e) \<in> set xs \<or> (\<exists> mo . Deliver (i, Expunge e mo i) \<in> set xs) \<or> (\<exists> mo . Deliver (i, Store e mo i) \<in> set xs)"
+  shows "Deliver (i, Create i e) \<in> set xs \<or> 
+    Deliver (i, Append i e) \<in> set xs \<or> 
+    (\<exists> mo . Deliver (i, Expunge e mo i) \<in> set xs) \<or> 
+    (\<exists> mo . Deliver (i, Store e mo i) \<in> set xs)"
 proof -  
   obtain y where "apply_operations xs = Some y"
     using assms broadcast_only_valid_msgs by blast
@@ -71,104 +77,107 @@ qed
   
 lemma (in imap) ids_are_unique:
     assumes "xs prefix of j"
-    and "(i, Add i e1) \<in> set (node_deliver_messages xs)" 
+    and "(i, Create i e1) \<in> set (node_deliver_messages xs)" 
     and "(l, Append l e2) \<in> set (node_deliver_messages xs)"
     and "(k, Expunge e3 mo k) \<in> set (node_deliver_messages xs)"
     and "(m, Store e4 mo2 m) \<in> set (node_deliver_messages xs)"
   shows "i \<noteq> l \<and> i \<noteq> k \<and> l \<noteq> k \<and> i \<noteq> m \<and> l \<noteq> m \<and> k \<noteq> m"
-  	using assms delivery_has_a_cause events_before_exist prefix_msg_in_history
-  	by (metis fst_conv msg_id_unique operation.distinct(15) operation.distinct(17) operation.distinct(19) operation.distinct(3) operation.distinct(5) operation.distinct(7) prod.inject) 
-  		
-lemma (in imap) concurrent_add_remove_independent_technical:
+    using assms delivery_has_a_cause events_before_exist prefix_msg_in_history
+    by (metis fst_conv msg_id_unique operation.distinct(15) operation.distinct(17) operation.distinct(19) operation.distinct(3) operation.distinct(5) operation.distinct(7) prod.inject) 
+      
+lemma (in imap) concurrent_create_delete_independent_technical:
   assumes "i \<in> is"
     and "xs prefix of j"
-    and "(i, Add i e) \<in> set (node_deliver_messages xs)" and "(ir, Rem is e) \<in> set (node_deliver_messages xs)"
-  shows "hb (i, Add i e) (ir, Rem is e)"
+    and "(i, Create i e) \<in> set (node_deliver_messages xs)" 
+    and "(ir, Delete is e) \<in> set (node_deliver_messages xs)"
+  shows "hb (i, Create i e) (ir, Delete is e)"
 proof -
-  obtain pre k where P: "pre@[Broadcast (ir, Rem is e)] prefix of k"
+  obtain pre k where P: "pre@[Broadcast (ir, Delete is e)] prefix of k"
     using assms delivery_has_a_cause events_before_exist prefix_msg_in_history by blast
-  hence "pre prefix of k"	by blast
-  moreover hence "Deliver (i, Add i e) \<in> set pre \<or> Deliver (i, Append i e) \<in> set pre \<or> (\<exists> mo . Deliver (i, Expunge e mo i) \<in> set pre) \<or> (\<exists> mo . Deliver (i, Store e mo i) \<in> set pre)"
-    using Broadcast_Deliver_prefix_closed assms(1) P by auto    	
-  hence "Deliver (i, Add i e) \<in> set pre" using network.msg_id_unique network.delivery_has_a_cause using assms(2) assms(3) ids_are_unique P
+  hence "pre prefix of k" by blast
+  moreover hence "Deliver (i, Create i e) \<in> set pre \<or> Deliver (i, Append i e) \<in> set pre \<or> (\<exists> mo . Deliver (i, Expunge e mo i) \<in> set pre) \<or> (\<exists> mo . Deliver (i, Store e mo i) \<in> set pre)"
+    using Broadcast_Deliver_prefix_closed assms(1) P by auto      
+  hence "Deliver (i, Create i e) \<in> set pre" using network.msg_id_unique network.delivery_has_a_cause using assms(2) assms(3) ids_are_unique P
   proof -
-  	obtain aa :: 'a and aaa :: 'a where
-  		f1: "(Deliver (i, Append i e) \<in> set pre \<or> (\<exists>a. Deliver (i, Expunge e a i) \<in> set pre) \<or> (\<exists>a. Deliver (i, Store e a i) \<in> set pre)) = (Deliver (i, Append i e) \<in> set pre \<or> Deliver (i, Expunge e aaa i) \<in> set pre \<or> Deliver (i, Store e aa i) \<in> set pre)"
-  		by blast
-  	have f2: "\<forall>p n pa na. Broadcast p \<notin> set (history n) \<or> Broadcast pa \<notin> set (history na) \<or> fst p \<noteq> fst pa \<or> n = na \<and> p = pa"
-  		using msg_id_unique by presburger
-  	obtain nn :: "'a \<times> ('a, 'b) operation \<Rightarrow> nat" where
-  		f3: "\<forall>p n. Deliver p \<notin> set (history n) \<or> Broadcast p \<in> set (history (nn p))"
-  		by (metis (no_types) delivery_has_a_cause)
-		then have f4: "Broadcast (i, Add i e) \<in> set (history (nn (i, Add i e)))"
-			using assms(2) assms(3) prefix_msg_in_history by blast
-		have f5: "\<forall>es n e. \<not> es prefix of n \<or> e \<notin> set es \<or> e \<in> set (history n)"
-			using prefix_elem_to_carriers by blast
-		then have f6: "Deliver (i, Append i e) \<in> set pre \<longrightarrow> nn (i, Append i e) = nn (i, Add i e) \<and> (i, Append i e) = (i, Add i e)"
-			using f4 f3 f2 by (metis (no_types) calculation fst_conv)
-		have f7: "Deliver (i, Expunge e aaa i) \<in> set pre \<longrightarrow> nn (i, Expunge e aaa i) = nn (i, Add i e) \<and> (i, Expunge e aaa i) = (i, Add i e)"
-			using f5 f4 f3 f2 by (metis (no_types) calculation fst_conv)
-		have "Deliver (i, Store e aa i) \<in> set pre \<longrightarrow> Deliver (i, Add i e) \<in> set pre"
-			using f5 f4 f3 f2 by (metis (no_types) calculation fst_conv)
-		then show ?thesis
-			using f7 f6 f1 \<open>Deliver (i, Add i e) \<in> set pre \<or> Deliver (i, Append i e) \<in> set pre \<or> (\<exists>mo. Deliver (i, Expunge e mo i) \<in> set pre) \<or> (\<exists>mo. Deliver (i, Store e mo i) \<in> set pre)\<close> by blast
-	qed  	
+    obtain aa :: 'a and aaa :: 'a where
+      f1: "(Deliver (i, Append i e) \<in> set pre \<or> (\<exists>a. Deliver (i, Expunge e a i) \<in> set pre) \<or> (\<exists>a. Deliver (i, Store e a i) \<in> set pre)) = (Deliver (i, Append i e) \<in> set pre \<or> Deliver (i, Expunge e aaa i) \<in> set pre \<or> Deliver (i, Store e aa i) \<in> set pre)"
+      by blast
+    have f2: "\<forall>p n pa na. Broadcast p \<notin> set (history n) \<or> Broadcast pa \<notin> set (history na) \<or> fst p \<noteq> fst pa \<or> n = na \<and> p = pa"
+      using msg_id_unique by presburger
+    obtain nn :: "'a \<times> ('a, 'b) operation \<Rightarrow> nat" where
+      f3: "\<forall>p n. Deliver p \<notin> set (history n) \<or> Broadcast p \<in> set (history (nn p))"
+      by (metis (no_types) delivery_has_a_cause)
+    then have f4: "Broadcast (i, Create i e) \<in> set (history (nn (i, Create i e)))"
+      using assms(2) assms(3) prefix_msg_in_history by blast
+    have f5: "\<forall>es n e. \<not> es prefix of n \<or> e \<notin> set es \<or> e \<in> set (history n)"
+      using prefix_elem_to_carriers by blast
+    then have f6: "Deliver (i, Append i e) \<in> set pre \<longrightarrow> nn (i, Append i e) = nn (i, Create i e) \<and> (i, Append i e) = (i, Create i e)"
+      using f4 f3 f2 by (metis (no_types) calculation fst_conv)
+    have f7: "Deliver (i, Expunge e aaa i) \<in> set pre \<longrightarrow> nn (i, Expunge e aaa i) = nn (i, Create i e) \<and> (i, Expunge e aaa i) = (i, Create i e)"
+      using f5 f4 f3 f2 by (metis (no_types) calculation fst_conv)
+    have "Deliver (i, Store e aa i) \<in> set pre \<longrightarrow> Deliver (i, Create i e) \<in> set pre"
+      using f5 f4 f3 f2 by (metis (no_types) calculation fst_conv)
+    then show ?thesis
+      using f7 f6 f1 \<open>Deliver (i, Create i e) \<in> set pre \<or> Deliver (i, Append i e) \<in> set pre \<or> (\<exists>mo. Deliver (i, Expunge e mo i) \<in> set pre) \<or> (\<exists>mo. Deliver (i, Store e mo i) \<in> set pre)\<close> by blast
+  qed   
   ultimately show ?thesis
     using hb.intros(2) events_in_local_order P by blast
 qed
 
-lemma (in imap) concurrent_append_remove_independent_technical:
+lemma (in imap) concurrent_append_delete_independent_technical:
   assumes "i \<in> is"
     and "xs prefix of j"
-    and "(i, Append i e) \<in> set (node_deliver_messages xs)" and "(ir, Rem is e) \<in> set (node_deliver_messages xs)"
-  shows "hb (i, Append i e) (ir, Rem is e)"
+    and "(i, Append i e) \<in> set (node_deliver_messages xs)" 
+    and "(ir, Delete is e) \<in> set (node_deliver_messages xs)"
+  shows "hb (i, Append i e) (ir, Delete is e)"
 proof -
-  obtain pre k where "pre@[Broadcast (ir, Rem is e)] prefix of k"
+  obtain pre k where "pre@[Broadcast (ir, Delete is e)] prefix of k"
     using assms delivery_has_a_cause events_before_exist prefix_msg_in_history by blast
-  moreover hence "Deliver (i, Add i e) \<in> set pre \<or> Deliver (i, Append i e) \<in> set pre \<or> (\<exists> mo . Deliver (i, Expunge e mo i) \<in> set pre) \<or> (\<exists> mo . Deliver (i, Store e mo i) \<in> set pre)"
+  moreover hence "Deliver (i, Create i e) \<in> set pre \<or> Deliver (i, Append i e) \<in> set pre \<or> (\<exists> mo . Deliver (i, Expunge e mo i) \<in> set pre) \<or> (\<exists> mo . Deliver (i, Store e mo i) \<in> set pre)"
     using Broadcast_Deliver_prefix_closed assms(1) by auto
-    	
+      
   hence "Deliver (i, Append i e) \<in> set pre" using assms ids_are_unique
   proof -
-  	have "pre prefix of k"
-  		using calculation by blast
-  	then have "\<And>e. e \<notin> set pre \<or> e \<in> set (history k)"
-  		by (simp add: node_histories.prefix_elem_to_carriers node_histories_axioms)
-  	then have "\<And>p. Deliver p \<notin> set pre \<or> fst p \<noteq> i \<or> p = (i, Append i e)"
-  		by (metis (no_types) \<open>(i, Append i e) \<in> set (node_deliver_messages xs)\<close> \<open>xs prefix of j\<close> delivery_has_a_cause fst_conv msg_id_unique prefix_msg_in_history)
-  	then show ?thesis
-  		using \<open>Deliver (i, Add i e) \<in> set pre \<or> Deliver (i, Append i e) \<in> set pre \<or> (\<exists>mo. Deliver (i, Expunge e mo i) \<in> set pre) \<or> (\<exists>mo. Deliver (i, Store e mo i) \<in> set pre)\<close> by fastforce
+    have "pre prefix of k"
+      using calculation by blast
+    then have "\<And>e. e \<notin> set pre \<or> e \<in> set (history k)"
+      by (simp add: node_histories.prefix_elem_to_carriers node_histories_axioms)
+    then have "\<And>p. Deliver p \<notin> set pre \<or> fst p \<noteq> i \<or> p = (i, Append i e)"
+      by (metis (no_types) \<open>(i, Append i e) \<in> set (node_deliver_messages xs)\<close> \<open>xs prefix of j\<close> delivery_has_a_cause fst_conv msg_id_unique prefix_msg_in_history)
+    then show ?thesis
+      using \<open>Deliver (i, Create i e) \<in> set pre \<or> Deliver (i, Append i e) \<in> set pre \<or> (\<exists>mo. Deliver (i, Expunge e mo i) \<in> set pre) \<or> (\<exists>mo. Deliver (i, Store e mo i) \<in> set pre)\<close> by fastforce
   qed 
     ultimately show ?thesis
     using hb.intros(2) events_in_local_order by blast
 qed
-	
+  
 lemma (in imap) concurrent_append_expunge_independent_technical:
   assumes "i = mo"
     and "xs prefix of j"
-    and "(i, Append i e) \<in> set (node_deliver_messages xs)" and "(r, Expunge e mo r) \<in> set (node_deliver_messages xs)"
+    and "(i, Append i e) \<in> set (node_deliver_messages xs)" 
+    and "(r, Expunge e mo r) \<in> set (node_deliver_messages xs)"
   shows "hb (i, Append i e) (r, Expunge e mo r)"
 proof -
   obtain pre k where "pre@[Broadcast (r, Expunge e mo r)] prefix of k"
     using assms delivery_has_a_cause events_before_exist prefix_msg_in_history by blast
   moreover hence "Deliver (mo, Append mo e) \<in> set pre \<or> (\<exists> mo2 . Deliver (mo, Store e mo2 mo) \<in> set pre)"
     using Broadcast_Expunge_Deliver_prefix_closed assms(1) by auto
-    	
+      
   hence "Deliver (i, Append i e) \<in> set pre" using assms assms ids_are_unique
   proof -
-  	obtain aa :: 'a where
-  		f1: "Deliver (mo, Append mo e) \<in> set pre \<or> Deliver (mo, Store e aa mo) \<in> set pre"
-  		using \<open>Deliver (mo, Append mo e) \<in> set pre \<or> (\<exists>mo2. Deliver (mo, Store e mo2 mo) \<in> set pre)\<close> by blast
-  	have f2: "Deliver (mo, Append mo e) \<in> set (history j)"
-  		using \<open>(i, Append i e) \<in> set (node_deliver_messages xs)\<close> \<open>i = mo\<close> \<open>xs prefix of j\<close> prefix_msg_in_history by blast
-  	{ assume "Deliver (mo, Store e aa mo) \<in> set pre"
-  		{ assume "v2_1 (mo, Store e aa mo) \<noteq> (v2_1 (mo, Append mo e)::nat) \<or> (mo, Store e aa mo) \<noteq> (mo, Append mo e)"
-  			then have "Deliver (mo, Store e aa mo) \<notin> set pre"
-  				using f2 by (metis (no_types) calculation delivery_has_a_cause fst_conv msg_id_unique prefix_elem_to_carriers prefix_of_appendD) }
-  		then have "Deliver (mo, Store e aa mo) \<in> set pre \<longrightarrow> Deliver (i, Append i e) \<in> set pre"
-  			by blast }
-  	then show ?thesis
-  		using f1 \<open>i = mo\<close> by blast
+    obtain aa :: 'a where
+      f1: "Deliver (mo, Append mo e) \<in> set pre \<or> Deliver (mo, Store e aa mo) \<in> set pre"
+      using \<open>Deliver (mo, Append mo e) \<in> set pre \<or> (\<exists>mo2. Deliver (mo, Store e mo2 mo) \<in> set pre)\<close> by blast
+    have f2: "Deliver (mo, Append mo e) \<in> set (history j)"
+      using \<open>(i, Append i e) \<in> set (node_deliver_messages xs)\<close> \<open>i = mo\<close> \<open>xs prefix of j\<close> prefix_msg_in_history by blast
+    { assume "Deliver (mo, Store e aa mo) \<in> set pre"
+      { assume "v2_1 (mo, Store e aa mo) \<noteq> (v2_1 (mo, Append mo e)::nat) \<or> (mo, Store e aa mo) \<noteq> (mo, Append mo e)"
+        then have "Deliver (mo, Store e aa mo) \<notin> set pre"
+          using f2 by (metis (no_types) calculation delivery_has_a_cause fst_conv msg_id_unique prefix_elem_to_carriers prefix_of_appendD) }
+      then have "Deliver (mo, Store e aa mo) \<in> set pre \<longrightarrow> Deliver (i, Append i e) \<in> set pre"
+        by blast }
+    then show ?thesis
+      using f1 \<open>i = mo\<close> by blast
   qed
   ultimately show ?thesis
     using hb.intros(2) events_in_local_order by blast
@@ -177,88 +186,84 @@ qed
 lemma (in imap) concurrent_append_store_independent_technical:
   assumes "i = mo"
     and "xs prefix of j"
-    and "(i, Append i e) \<in> set (node_deliver_messages xs)" and "(r, Store e mo r) \<in> set (node_deliver_messages xs)"
+    and "(i, Append i e) \<in> set (node_deliver_messages xs)" 
+    and "(r, Store e mo r) \<in> set (node_deliver_messages xs)"
   shows "hb (i, Append i e) (r, Store e mo r)"
 proof -
   obtain pre k where "pre@[Broadcast (r, Store e mo r)] prefix of k"
     using assms delivery_has_a_cause events_before_exist prefix_msg_in_history by blast
   moreover hence A: "Deliver (mo, Append mo e) \<in> set pre \<or> (\<exists> mo2 . Deliver (mo, Store e mo2 mo) \<in> set pre)"
-    using Broadcast_Store_Deliver_prefix_closed assms(1) by auto
-    	
+    using Broadcast_Store_Deliver_prefix_closed assms(1) by auto      
   hence "Deliver (i, Append i e) \<in> set pre" using assms ids_are_unique
   proof -
-  	have f1: "Deliver (i, Append i e) \<in> set (history j)"
-  		by (meson assms network.prefix_msg_in_history network_axioms)
-  	obtain aa :: 'a where
-  		"Deliver (i, Append i e) \<in> set pre \<or> Deliver (i, Store e aa i) \<in> set pre"
-  		using A assms by blast
-  	then show ?thesis
-  		using f1 by (metis (no_types) calculation delivery_has_a_cause fst_conv msg_id_unique prefix_elem_to_carriers prefix_of_appendD)
+    have f1: "Deliver (i, Append i e) \<in> set (history j)"
+      by (meson assms network.prefix_msg_in_history network_axioms)
+    obtain aa :: 'a where
+      "Deliver (i, Append i e) \<in> set pre \<or> Deliver (i, Store e aa i) \<in> set pre"
+      using A assms by blast
+    then show ?thesis
+      using f1 by (metis (no_types) calculation delivery_has_a_cause fst_conv msg_id_unique prefix_elem_to_carriers prefix_of_appendD)
   qed
-
   ultimately show ?thesis
     using hb.intros(2) events_in_local_order by blast
 qed
   
-
-	
-lemma (in imap) concurrent_store_remove_independent_technical:
+lemma (in imap) concurrent_store_delete_independent_technical:
   assumes "i \<in> is"
     and "xs prefix of j"
-    and "(i, Store e mo i) \<in> set (node_deliver_messages xs)" and "(ir, Rem is e) \<in> set (node_deliver_messages xs)"
-  shows "hb (i, Store e mo i) (ir, Rem is e)"
+    and "(i, Store e mo i) \<in> set (node_deliver_messages xs)" 
+    and "(ir, Delete is e) \<in> set (node_deliver_messages xs)"
+  shows "hb (i, Store e mo i) (ir, Delete is e)"
 proof -
-  obtain pre k where P: "pre@[Broadcast (ir, Rem is e)] prefix of k"
+  obtain pre k where P: "pre@[Broadcast (ir, Delete is e)] prefix of k"
     using assms delivery_has_a_cause events_before_exist prefix_msg_in_history by blast
-  moreover hence A: "Deliver (i, Add i e) \<in> set pre \<or> Deliver (i, Append i e) \<in> set pre \<or> (\<exists> mo . Deliver (i, Expunge e mo i) \<in> set pre) \<or> (\<exists> mo . Deliver (i, Store e mo i) \<in> set pre)"
-    using Broadcast_Deliver_prefix_closed assms(1) by auto
-    	
+  moreover hence A: "Deliver (i, Create i e) \<in> set pre \<or> Deliver (i, Append i e) \<in> set pre \<or> (\<exists> mo . Deliver (i, Expunge e mo i) \<in> set pre) \<or> (\<exists> mo . Deliver (i, Store e mo i) \<in> set pre)"
+    using Broadcast_Deliver_prefix_closed assms(1) by auto      
   hence "Deliver (i, Store e mo i) \<in> set pre" using assms ids_are_unique P 
   proof -
-  	have "pre prefix of k"
-  		using calculation by blast
-  	then have "\<And>e. \<not> node_histories history \<or> e \<notin> set pre \<or> e \<in> set (history k)"
-  		by (simp add: node_histories.prefix_elem_to_carriers)
-  	then have f1: "\<And>e. e \<notin> set pre \<or> e \<in> set (history k)"
-  		using node_histories_axioms by blast
-  	have "\<And>f. \<not> network history (f::'a \<times> ('a, 'b) operation \<Rightarrow> 'a) \<or> Deliver (i, Store e mo i) \<in> set (history j)"
-  		by (meson assms network.prefix_msg_in_history)
-  	then have f2: "Deliver (i, Store e mo i) \<in> set (history j)"
-  		using network_axioms by blast
-  	obtain nn :: "'a \<times> ('a, 'b) operation \<Rightarrow> nat" where
-  		f3: "\<And>p n. Deliver p \<notin> set (history n) \<or> Broadcast p \<in> set (history (nn p))"
-  		by (metis delivery_has_a_cause)
-  	then have f4: "Broadcast (i, Store e mo i) \<in> set (history (nn (i, Store e mo i)))"
-  		using f2 by blast
-		have "\<And>p. Deliver p \<notin> set pre \<or> Broadcast p \<in> set (history (nn p))"
-			using f3 f1 by blast
-		then show ?thesis
-			using f4 by (metis (no_types) A fst_conv msg_id_unique)
-	qed
-  		
+    have "pre prefix of k"
+      using calculation by blast
+    then have "\<And>e. \<not> node_histories history \<or> e \<notin> set pre \<or> e \<in> set (history k)"
+      by (simp add: node_histories.prefix_elem_to_carriers)
+    then have f1: "\<And>e. e \<notin> set pre \<or> e \<in> set (history k)"
+      using node_histories_axioms by blast
+    have "\<And>f. \<not> network history (f::'a \<times> ('a, 'b) operation \<Rightarrow> 'a) \<or> Deliver (i, Store e mo i) \<in> set (history j)"
+      by (meson assms network.prefix_msg_in_history)
+    then have f2: "Deliver (i, Store e mo i) \<in> set (history j)"
+      using network_axioms by blast
+    obtain nn :: "'a \<times> ('a, 'b) operation \<Rightarrow> nat" where
+      f3: "\<And>p n. Deliver p \<notin> set (history n) \<or> Broadcast p \<in> set (history (nn p))"
+      by (metis delivery_has_a_cause)
+    then have f4: "Broadcast (i, Store e mo i) \<in> set (history (nn (i, Store e mo i)))"
+      using f2 by blast
+    have "\<And>p. Deliver p \<notin> set pre \<or> Broadcast p \<in> set (history (nn p))"
+      using f3 f1 by blast
+    then show ?thesis
+      using f4 by (metis (no_types) A fst_conv msg_id_unique)
+  qed      
   ultimately show ?thesis
     using hb.intros(2) events_in_local_order by blast
 qed
-	
+  
 lemma (in imap) concurrent_store_expunge_independent_technical:
     assumes "xs prefix of j"
-    and "(i, Store e mo i) \<in> set (node_deliver_messages xs)" and "(r, Expunge e i r) \<in> set (node_deliver_messages xs)"
+    and "(i, Store e mo i) \<in> set (node_deliver_messages xs)" 
+    and "(r, Expunge e i r) \<in> set (node_deliver_messages xs)"
   shows "hb (i, Store e mo i) (r, Expunge e i r)"
 proof -
   obtain pre k where "pre@[Broadcast (r, Expunge e i r)] prefix of k"
     using assms delivery_has_a_cause events_before_exist prefix_msg_in_history by blast
   moreover hence A: "Deliver (i, Append i e) \<in> set pre \<or> (\<exists> mo2 . Deliver (i, Store e mo2 i) \<in> set pre)"
-    using Broadcast_Expunge_Deliver_prefix_closed assms(1) by auto
-    	
+    using Broadcast_Expunge_Deliver_prefix_closed assms(1) by auto      
   hence "Deliver (i, Store e mo i) \<in> set pre" using assms ids_are_unique
   proof -
-  	obtain aa :: 'a where
-  		f1: "Deliver (i, Append i e) \<in> set pre \<or> Deliver (i, Store e aa i) \<in> set pre"
-  		using A by blast
-  	obtain nn :: "'a \<times> ('a, 'b) operation \<Rightarrow> nat" where
-  				f2: "\<forall>p. (\<forall>n. Deliver p \<notin> set (history n)) \<or> Broadcast p \<in> set (history (nn p))"
-  		by (metis (no_types) delivery_has_a_cause)
-  	have f3: "\<And>e. e \<in> set (history k) \<or> e \<notin> set pre"
+    obtain aa :: 'a where
+      f1: "Deliver (i, Append i e) \<in> set pre \<or> Deliver (i, Store e aa i) \<in> set pre"
+      using A by blast
+    obtain nn :: "'a \<times> ('a, 'b) operation \<Rightarrow> nat" where
+          f2: "\<forall>p. (\<forall>n. Deliver p \<notin> set (history n)) \<or> Broadcast p \<in> set (history (nn p))"
+      by (metis (no_types) delivery_has_a_cause)
+    have f3: "\<And>e. e \<in> set (history k) \<or> e \<notin> set pre"
     using calculation prefix_elem_to_carriers by blast
   have f4: "\<And>z n. (i, z) = (i, Store e mo i) \<or> Broadcast (i, z) \<notin> set (history n)"
     using f2 by (metis assms(1) assms(2) fst_conv msg_id_unique prefix_msg_in_history)
@@ -269,15 +274,15 @@ proof -
       using f4 f3 f2 f1 by blast }
   then show ?thesis
     by blast
-	qed 
-  		
+  qed      
   ultimately show ?thesis
     using hb.intros(2) events_in_local_order by blast
 qed
-	
+  
 lemma (in imap) concurrent_store_expunge_independent_technical2:
     assumes "xs prefix of j"
-    and "(i, Store e1 mo2 i) \<in> set (node_deliver_messages xs)" and "(r, Expunge e mo r) \<in> set (node_deliver_messages xs)"
+    and "(i, Store e1 mo2 i) \<in> set (node_deliver_messages xs)" 
+    and "(r, Expunge e mo r) \<in> set (node_deliver_messages xs)"
   shows "mo2 \<noteq> r"
 proof -
   obtain nn :: "'a \<times> ('a, 'b) operation \<Rightarrow> nat" where
@@ -305,160 +310,160 @@ proof -
   then show ?thesis
     using f7 f6 f5 f4 f3 f1
   proof -
-  	obtain aaa :: "'a \<Rightarrow> 'b \<Rightarrow> ('a \<times> ('a, 'b) operation) event list \<Rightarrow> 'a" where
-  		x1: "\<forall>x1 x2 x4. (\<exists>v6. Deliver (x1, Store x2 v6 x1) \<in> set x4) = (Deliver (x1, Store x2 (aaa x1 x2 x4) x1) \<in> set x4)"
-  		by moura
-  	obtain eesa :: "nat \<Rightarrow> ('a \<times> ('a, 'b) operation) event \<Rightarrow> ('a \<times> ('a, 'b) operation) event list" where
-  		"\<forall>x0 x1. (\<exists>v2. v2 @ [x1] prefix of x0) = (eesa x0 x1 @ [x1] prefix of x0)"
-  		by moura
-  	then have x2: "\<forall>e n. e \<notin> set (history n) \<or> eesa n e @ [e] prefix of n"
-  		using events_before_exist by presburger
-  	then have x3: "eesa (nn (i, Store e1 mo2 i)) (Broadcast (i, Store e1 mo2 i)) prefix of nn (i, Store e1 mo2 i)"
-  		using f1 f5 by blast
-  	have x4: "Deliver (r, Append r e1) \<notin> set (history (nn (i, Store e1 mo2 i)))"
-  		by (metis (no_types) f1 f2 fst_conv msg_id_unique old.prod.inject operation.distinct(15))
-  	have "Deliver (r, Store e1 (aaa r e1 (eesa (nn (i, Store e1 mo2 i)) (Broadcast (i, Store e1 mo2 i)))) r) \<notin> set (history (nn (i, Store e1 mo2 i)))"
-  		by (metis (no_types) f1 f2 fst_conv msg_id_unique old.prod.inject operation.distinct(19))
-  	then have "r \<noteq> mo2"
-  		using x4 x3 x2 x1 by (meson f1 f5 imap.Broadcast_Store_Deliver_prefix_closed imap_axioms prefix_elem_to_carriers)
-  	then show ?thesis
-  		by meson
+    obtain aaa :: "'a \<Rightarrow> 'b \<Rightarrow> ('a \<times> ('a, 'b) operation) event list \<Rightarrow> 'a" where
+      x1: "\<forall>x1 x2 x4. (\<exists>v6. Deliver (x1, Store x2 v6 x1) \<in> set x4) = (Deliver (x1, Store x2 (aaa x1 x2 x4) x1) \<in> set x4)"
+      by moura
+    obtain eesa :: "nat \<Rightarrow> ('a \<times> ('a, 'b) operation) event \<Rightarrow> ('a \<times> ('a, 'b) operation) event list" where
+      "\<forall>x0 x1. (\<exists>v2. v2 @ [x1] prefix of x0) = (eesa x0 x1 @ [x1] prefix of x0)"
+      by moura
+    then have x2: "\<forall>e n. e \<notin> set (history n) \<or> eesa n e @ [e] prefix of n"
+      using events_before_exist by presburger
+    then have x3: "eesa (nn (i, Store e1 mo2 i)) (Broadcast (i, Store e1 mo2 i)) prefix of nn (i, Store e1 mo2 i)"
+      using f1 f5 by blast
+    have x4: "Deliver (r, Append r e1) \<notin> set (history (nn (i, Store e1 mo2 i)))"
+      by (metis (no_types) f1 f2 fst_conv msg_id_unique old.prod.inject operation.distinct(15))
+    have "Deliver (r, Store e1 (aaa r e1 (eesa (nn (i, Store e1 mo2 i)) (Broadcast (i, Store e1 mo2 i)))) r) \<notin> set (history (nn (i, Store e1 mo2 i)))"
+      by (metis (no_types) f1 f2 fst_conv msg_id_unique old.prod.inject operation.distinct(19))
+    then have "r \<noteq> mo2"
+      using x4 x3 x2 x1 by (meson f1 f5 imap.Broadcast_Store_Deliver_prefix_closed imap_axioms prefix_elem_to_carriers)
+    then show ?thesis
+      by meson
   qed 
 qed
  
-lemma (in imap) concurrent_expunge_remove_independent_technical:
+lemma (in imap) concurrent_expunge_delete_independent_technical:
   assumes "i \<in> is"
     and "xs prefix of j"
-    and "(i, Expunge e mo i) \<in> set (node_deliver_messages xs)" and "(ir, Rem is e) \<in> set (node_deliver_messages xs)"
-  shows "hb (i, Expunge e mo i) (ir, Rem is e)"
+    and "(i, Expunge e mo i) \<in> set (node_deliver_messages xs)" 
+    and "(ir, Delete is e) \<in> set (node_deliver_messages xs)"
+  shows "hb (i, Expunge e mo i) (ir, Delete is e)"
 proof -
-  obtain pre k where "pre@[Broadcast (ir, Rem is e)] prefix of k"
+  obtain pre k where "pre@[Broadcast (ir, Delete is e)] prefix of k"
     using assms delivery_has_a_cause events_before_exist prefix_msg_in_history by blast
-  moreover hence A: "Deliver (i, Add i e) \<in> set pre \<or> Deliver (i, Append i e) \<in> set pre \<or> (\<exists> mo . Deliver (i, Expunge e mo i) \<in> set pre) \<or> (\<exists> mo . Deliver (i, Store e mo i) \<in> set pre)"
-    using Broadcast_Deliver_prefix_closed assms(1) by auto
-    	
+  moreover hence A: "Deliver (i, Create i e) \<in> set pre \<or> Deliver (i, Append i e) \<in> set pre \<or> (\<exists> mo . Deliver (i, Expunge e mo i) \<in> set pre) \<or> (\<exists> mo . Deliver (i, Store e mo i) \<in> set pre)"
+    using Broadcast_Deliver_prefix_closed assms(1) by auto      
   hence "Deliver (i, Expunge e mo i) \<in> set pre" using assms ids_are_unique
   proof -
-  	have "pre prefix of k"
-  		using calculation by blast
-  	then have f1: "\<And>e. e \<notin> set pre \<or> e \<in> set (history k)"
-  		by (simp add: node_histories.prefix_elem_to_carriers node_histories_axioms)
-  	have f2: "Deliver (i, Expunge e mo i) \<in> set (history j)"
-  		by (meson assms network.prefix_msg_in_history network_axioms)
-  	obtain nn :: "'a \<times> ('a, 'b) operation \<Rightarrow> nat" where
-  		"\<And>p n. Deliver p \<notin> set (history n) \<or> Broadcast p \<in> set (history (nn p))"
-  		by (metis (no_types) delivery_has_a_cause)
-  	then show ?thesis
-  		using f2 f1 by (metis (no_types) A fst_conv msg_id_unique)
-  qed  		
+    have "pre prefix of k"
+      using calculation by blast
+    then have f1: "\<And>e. e \<notin> set pre \<or> e \<in> set (history k)"
+      by (simp add: node_histories.prefix_elem_to_carriers node_histories_axioms)
+    have f2: "Deliver (i, Expunge e mo i) \<in> set (history j)"
+      by (meson assms network.prefix_msg_in_history network_axioms)
+    obtain nn :: "'a \<times> ('a, 'b) operation \<Rightarrow> nat" where
+      "\<And>p n. Deliver p \<notin> set (history n) \<or> Broadcast p \<in> set (history (nn p))"
+      by (metis (no_types) delivery_has_a_cause)
+    then show ?thesis
+      using f2 f1 by (metis (no_types) A fst_conv msg_id_unique)
+  qed     
   ultimately show ?thesis
     using hb.intros(2) events_in_local_order by blast
 qed
-	
+  
 lemma (in imap) concurrent_store_store_independent_technical:
-    assumes "xs prefix of j"
-    and "(i, Store e mo i) \<in> set (node_deliver_messages xs)" and "(r, Store e i r) \<in> set (node_deliver_messages xs)"
+  assumes "xs prefix of j"
+    and "(i, Store e mo i) \<in> set (node_deliver_messages xs)" 
+    and "(r, Store e i r) \<in> set (node_deliver_messages xs)"
   shows "hb (i, Store e mo i) (r, Store e i r)"
 proof -
   obtain pre k where "pre@[Broadcast (r, Store e i r)] prefix of k"
     using assms delivery_has_a_cause events_before_exist prefix_msg_in_history by blast
   moreover hence A: "Deliver (i, Append i e) \<in> set pre \<or> (\<exists> mo2 . Deliver (i, Store e mo2 i) \<in> set pre)"
-    using Broadcast_Store_Deliver_prefix_closed assms(1) by auto
-    	
+    using Broadcast_Store_Deliver_prefix_closed assms(1) by auto      
   hence "Deliver (i, Store e mo i) \<in> set pre" using assms ids_are_unique
   proof -
-  	have "\<forall>e. e \<notin> set pre \<or> e \<in> set (history k)"
-  		by (meson calculation node_histories.prefix_of_appendD node_histories_axioms prefix_to_carriers subset_iff)
-  	then show ?thesis
-  		by (metis (no_types) A assms(1) assms(2) delivery_has_a_cause fst_conv msg_id_unique prefix_msg_in_history)
-  qed  		
+    have "\<forall>e. e \<notin> set pre \<or> e \<in> set (history k)"
+      by (meson calculation node_histories.prefix_of_appendD node_histories_axioms prefix_to_carriers subset_iff)
+    then show ?thesis
+      by (metis (no_types) A assms(1) assms(2) delivery_has_a_cause fst_conv msg_id_unique prefix_msg_in_history)
+  qed     
   ultimately show ?thesis
     using hb.intros(2) events_in_local_order by blast
 qed 
-	
-	
-lemma (in imap) expunge_rem_ids_imply_messages_same:
+  
+  
+lemma (in imap) expunge_delete_ids_imply_messages_same:
   assumes "i \<in> is"
     and "xs prefix of j"
-    and "(i, Expunge e1 mo i) \<in> set (node_deliver_messages xs)" and "(ir, Rem is e2) \<in> set (node_deliver_messages xs)"
+    and "(i, Expunge e1 mo i) \<in> set (node_deliver_messages xs)" 
+    and "(ir, Delete is e2) \<in> set (node_deliver_messages xs)"
   shows "e1 = e2"
 proof -
-  obtain pre k where P: "pre@[Broadcast (ir, Rem is e2)] prefix of k"
+  obtain pre k where P: "pre@[Broadcast (ir, Delete is e2)] prefix of k"
     using assms delivery_has_a_cause events_before_exist prefix_msg_in_history by blast  
-   moreover hence A: "Deliver (i, Add i e2) \<in> set pre \<or> Deliver (i, Append i e2) \<in> set pre \<or> (\<exists> mo . Deliver (i, Expunge e2 mo i) \<in> set pre) \<or> (\<exists> mo . Deliver (i, Store e2 mo i) \<in> set pre)"
-   	 using Broadcast_Deliver_prefix_closed assms(1) by (meson imap.Broadcast_Deliver_prefix_closed imap_axioms)  
+   moreover hence A: "Deliver (i, Create i e2) \<in> set pre \<or> Deliver (i, Append i e2) \<in> set pre \<or> (\<exists> mo . Deliver (i, Expunge e2 mo i) \<in> set pre) \<or> (\<exists> mo . Deliver (i, Store e2 mo i) \<in> set pre)"
+     using Broadcast_Deliver_prefix_closed assms(1) by (meson imap.Broadcast_Deliver_prefix_closed imap_axioms)  
   hence "Deliver (i, Expunge e2 mo i) \<in> set pre" using assms ids_are_unique
   proof -
-  	have "pre prefix of k"
-  		using calculation by blast
-  	then have f1: "\<And>e2. e2 \<notin> set pre \<or> e2 \<in> set (history k)"
-  		by (simp add: node_histories.prefix_elem_to_carriers node_histories_axioms)
-  	have f2: "Deliver (i, Expunge e2 mo i) \<in> set (history j)"
-  		using assms A P network.prefix_msg_in_history network_axioms
-  	proof -
-  		have f1: "\<forall>es n e. \<not> es prefix of n \<or> e \<notin> set es \<or> e \<in> set (history n)"
-  			using prefix_elem_to_carriers by satx
-  		have f2: "i \<in> set (added_ids [Deliver (i, Expunge e1 mo i)] e1)"
-  			by simp
-  		have f3: "\<forall>a. (a::'a) \<notin> {}"
-  			by auto
-  		have f4: "\<forall>p n pa na. Broadcast p \<notin> set (history n) \<or> Broadcast pa \<notin> set (history na) \<or> fst p \<noteq> fst pa \<or> n = na \<and> p = pa"
-  			using msg_id_unique by presburger
-  		obtain nn :: "'a \<times> ('a, 'b) operation \<Rightarrow> nat" where
-  			f5: "\<forall>p n. Deliver p \<notin> set (history n) \<or> Broadcast p \<in> set (history (nn p))"
-  			by (metis (no_types) delivery_has_a_cause)
-  		then have f6: "Broadcast (i, Expunge e1 mo i) \<in> set (history (nn (i, Expunge e1 mo i)))"
-  			using assms(2) assms(3) prefix_msg_in_history by blast
-  		then have "Deliver (i, Append i e2) \<notin> set (history k)"
-  			using f5 f4 f3 f2 by (metis (no_types) added_files_Deliver_Append_same_collapse added_files_Deliver_Expunge_collapse added_ids_Deliver_Expunge_same_collapse empty_set fst_conv)
-  		then obtain aa :: 'a and aaa :: 'a where
-  					f7: "Deliver (i, Add i e2) \<in> set pre \<or> Deliver (i, Expunge e2 aaa i) \<in> set pre \<or> Deliver (i, Store e2 aa i) \<in> set pre"
-  			using f1 A \<open>pre prefix of k\<close> by blast
-  		have f8: "Deliver (i, Store e2 aa i) \<notin> set pre"
-  			using f6 f5 f4 f3 f2 f1 by (metis \<open>pre prefix of k\<close> added_files_Deliver_Expunge_collapse added_files_Deliver_Store_same_collapse added_ids_Deliver_Expunge_same_collapse empty_set fst_conv)
-  		have "added_ids [Deliver (i, Add i e2)] e1 \<noteq> [] \<or> (i, Add i e2) \<noteq> (i, Expunge e1 mo i)"
-  			by fastforce
-  		then have "e2 = e1"
-  			using f8 f7 f6 f5 f4 f3 f1 by (metis \<open>pre prefix of k\<close> added_ids_Deliver_Add_diff_collapse added_ids_Deliver_Expunge_diff_collapse empty_set expunge_id_not_in_set fst_conv)
-  		then show ?thesis
-  			by (meson assms(2) assms(3) network.prefix_msg_in_history network_axioms)
-  	qed 
-  	obtain nn :: "'a \<times> ('a, 'b) operation \<Rightarrow> nat" where
-  		"\<And>p n. Deliver p \<notin> set (history n) \<or> Broadcast p \<in> set (history (nn p))"
-  		by (metis (no_types) delivery_has_a_cause)
-  	then show ?thesis
-  		using f2 f1 by (metis (no_types) A fst_conv msg_id_unique)
-  qed  		
-  	moreover have "Deliver(i, Expunge e1 mo i) \<in> set (history j)"
+    have "pre prefix of k"
+      using calculation by blast
+    then have f1: "\<And>e2. e2 \<notin> set pre \<or> e2 \<in> set (history k)"
+      by (simp add: node_histories.prefix_elem_to_carriers node_histories_axioms)
+    have f2: "Deliver (i, Expunge e2 mo i) \<in> set (history j)"
+      using assms A P network.prefix_msg_in_history network_axioms
+    proof -
+      have f1: "\<forall>es n e. \<not> es prefix of n \<or> e \<notin> set es \<or> e \<in> set (history n)"
+        using prefix_elem_to_carriers by satx
+      have f2: "i \<in> set (added_ids [Deliver (i, Expunge e1 mo i)] e1)"
+        by simp
+      have f3: "\<forall>a. (a::'a) \<notin> {}"
+        by auto
+      have f4: "\<forall>p n pa na. Broadcast p \<notin> set (history n) \<or> Broadcast pa \<notin> set (history na) \<or> fst p \<noteq> fst pa \<or> n = na \<and> p = pa"
+        using msg_id_unique by presburger
+      obtain nn :: "'a \<times> ('a, 'b) operation \<Rightarrow> nat" where
+        f5: "\<forall>p n. Deliver p \<notin> set (history n) \<or> Broadcast p \<in> set (history (nn p))"
+        by (metis (no_types) delivery_has_a_cause)
+      then have f6: "Broadcast (i, Expunge e1 mo i) \<in> set (history (nn (i, Expunge e1 mo i)))"
+        using assms(2) assms(3) prefix_msg_in_history by blast
+      then have "Deliver (i, Append i e2) \<notin> set (history k)"
+        using f5 f4 f3 f2 by (metis (no_types) added_files_Deliver_Append_same_collapse added_files_Deliver_Expunge_collapse added_ids_Deliver_Expunge_same_collapse empty_set fst_conv)
+      then obtain aa :: 'a and aaa :: 'a where
+            f7: "Deliver (i, Create i e2) \<in> set pre \<or> Deliver (i, Expunge e2 aaa i) \<in> set pre \<or> Deliver (i, Store e2 aa i) \<in> set pre"
+        using f1 A \<open>pre prefix of k\<close> by blast
+      have f8: "Deliver (i, Store e2 aa i) \<notin> set pre"
+        using f6 f5 f4 f3 f2 f1 by (metis \<open>pre prefix of k\<close> added_files_Deliver_Expunge_collapse added_files_Deliver_Store_same_collapse added_ids_Deliver_Expunge_same_collapse empty_set fst_conv)
+      have "added_ids [Deliver (i, Create i e2)] e1 \<noteq> [] \<or> (i, Create i e2) \<noteq> (i, Expunge e1 mo i)"
+        by fastforce
+      then have "e2 = e1"
+        using f8 f7 f6 f5 f4 f3 f1 by (metis \<open>pre prefix of k\<close> added_ids_Deliver_Create_diff_collapse added_ids_Deliver_Expunge_diff_collapse empty_set expunge_id_not_in_set fst_conv)
+      then show ?thesis
+        by (meson assms(2) assms(3) network.prefix_msg_in_history network_axioms)
+    qed 
+    obtain nn :: "'a \<times> ('a, 'b) operation \<Rightarrow> nat" where
+      "\<And>p n. Deliver p \<notin> set (history n) \<or> Broadcast p \<in> set (history (nn p))"
+      by (metis (no_types) delivery_has_a_cause)
+    then show ?thesis
+      using f2 f1 by (metis (no_types) A fst_conv msg_id_unique)
+  qed     
+    moreover have "Deliver(i, Expunge e1 mo i) \<in> set (history j)"
     using assms(2) assms(3) prefix_msg_in_history by blast
   ultimately show ?thesis
     by (metis (no_types, lifting) delivery_has_a_cause fst_conv network.msg_id_unique network_axioms operation.inject(4) prefix_elem_to_carriers prefix_of_appendD prod.inject)
 qed
-	
-lemma (in imap) store_rem_ids_imply_messages_same:
+  
+lemma (in imap) store_delete_ids_imply_messages_same:
   assumes "i \<in> is"
     and "xs prefix of j"
-    and "(i, Store e1 mo i) \<in> set (node_deliver_messages xs)" and "(ir, Rem is e2) \<in> set (node_deliver_messages xs)"
+    and "(i, Store e1 mo i) \<in> set (node_deliver_messages xs)" 
+    and "(ir, Delete is e2) \<in> set (node_deliver_messages xs)"
   shows "e1 = e2"
 proof -
-  obtain pre k where P: "pre@[Broadcast (ir, Rem is e2)] prefix of k"
-    using assms delivery_has_a_cause events_before_exist prefix_msg_in_history by blast
-  
-   moreover hence A: "Deliver (i, Add i e2) \<in> set pre \<or> Deliver (i, Append i e2) \<in> set pre \<or> (\<exists> mo . Deliver (i, Expunge e2 mo i) \<in> set pre) \<or> (\<exists> mo . Deliver (i, Store e2 mo i) \<in> set pre)"
+  obtain pre k where P: "pre@[Broadcast (ir, Delete is e2)] prefix of k"
+    using assms delivery_has_a_cause events_before_exist prefix_msg_in_history by blast  
+   moreover hence A: "Deliver (i, Create i e2) \<in> set pre \<or> Deliver (i, Append i e2) \<in> set pre \<or> (\<exists> mo . Deliver (i, Expunge e2 mo i) \<in> set pre) \<or> (\<exists> mo . Deliver (i, Store e2 mo i) \<in> set pre)"
     using Broadcast_Deliver_prefix_closed assms(1)
-    by (meson imap.Broadcast_Deliver_prefix_closed imap_axioms)
-  		
+    by (meson imap.Broadcast_Deliver_prefix_closed imap_axioms)      
   hence "Deliver (i, Store e2 mo i) \<in> set pre" using assms ids_are_unique P 
   proof -
-  	have "pre prefix of k"
-  		using calculation by blast
-  	then have "\<And>e2. \<not> node_histories history \<or> e2 \<notin> set pre \<or> e2 \<in> set (history k)"
-  		by (simp add: node_histories.prefix_elem_to_carriers)
-  	then have f1: "\<And>e2. e2 \<notin> set pre \<or> e2 \<in> set (history k)"
-  		using node_histories_axioms by blast
-  	have "\<And>f. \<not> network history (f::'a \<times> ('a, 'b) operation \<Rightarrow> 'a) \<or> Deliver (i, Store e2 mo i) \<in> set (history j)"
-  		using assms network.prefix_msg_in_history P A
-  	proof -
+    have "pre prefix of k"
+      using calculation by blast
+    then have "\<And>e2. \<not> node_histories history \<or> e2 \<notin> set pre \<or> e2 \<in> set (history k)"
+      by (simp add: node_histories.prefix_elem_to_carriers)
+    then have f1: "\<And>e2. e2 \<notin> set pre \<or> e2 \<in> set (history k)"
+      using node_histories_axioms by blast
+    have "\<And>f. \<not> network history (f::'a \<times> ('a, 'b) operation \<Rightarrow> 'a) \<or> Deliver (i, Store e2 mo i) \<in> set (history j)"
+      using assms network.prefix_msg_in_history P A
+    proof -
   fix f :: "'a \<times> ('a, 'b) operation \<Rightarrow> 'a"
   have f1: "\<forall>a. (a::'a) \<notin> {}"
     by blast
@@ -470,146 +475,142 @@ proof -
   then have f4: "Broadcast (i, Store e1 mo i) \<in> set (history (nn (i, Store e1 mo i)))"
     using assms(2) assms(3) prefix_msg_in_history by blast
   obtain aa :: 'a and aaa :: 'a where
-    f5: "Deliver (i, Add i e2) \<in> set pre \<or> Deliver (i, Append i e2) \<in> set pre \<or> Deliver (i, Expunge e2 aaa i) \<in> set pre \<or> Deliver (i, Store e2 aa i) \<in> set pre"
+    f5: "Deliver (i, Create i e2) \<in> set pre \<or> Deliver (i, Append i e2) \<in> set pre \<or> Deliver (i, Expunge e2 aaa i) \<in> set pre \<or> Deliver (i, Store e2 aa i) \<in> set pre"
     using A by blast
   have f6: "Deliver (i, Store e2 aa i) \<in> set (history k) \<longrightarrow> [i] = added_files [Deliver (i, Store e1 mo i)] e2"
     using f4 f3 f2 by (metis (full_types) added_files_Deliver_Store_same_collapse fst_conv network_axioms)
   have "Deliver (i, Expunge e2 aaa i) \<notin> set (history k)"
     using f4 f3 f2 f1 by (metis (full_types) added_files_Deliver_Expunge_collapse added_files_Deliver_Store_same_collapse empty_set fst_conv list.set_intros(1) network_axioms)
   then have f7: "Deliver (i, Expunge e2 aaa i) \<notin> set pre"
-  		using \<open>pre prefix of k\<close> prefix_elem_to_carriers by blast
-  	have f8: "Deliver (i, Add i e2) \<notin> set (history k)"
-  		using f4 f3 f2 f1 by (metis (full_types) added_files_Deliver_Add_collapse added_files_Deliver_Store_same_collapse empty_set fst_conv list.set_intros(1) network_axioms)
-  	{ assume "added_files [Deliver (i, Store e1 mo i)] e2 = []"
-  		then have "Deliver (i, Append i e2) \<notin> set (history k)"
-  			using f4 f3 f2 f1 by (metis (full_types) added_files_Deliver_Append_same_collapse empty_set fst_conv list.set_intros(1) network_axioms)
-  		then have "e1 = e2"
-  			using f8 f7 f6 f5 f1 by (metis (no_types) \<open>pre prefix of k\<close> added_files_Deliver_Store_diff_collapse empty_set list.set_intros(1) prefix_elem_to_carriers) }
-  	then have "(i, Store e2 mo i) \<in> set (node_deliver_messages xs)"
-  		by (metis (no_types) added_files_Deliver_Store_diff_collapse assms(3))
-  	then show "\<not> network history f \<or> Deliver (i, Store e2 mo i) \<in> set (history j)"
-  		by (meson assms(2) network.prefix_msg_in_history)
+      using \<open>pre prefix of k\<close> prefix_elem_to_carriers by blast
+    have f8: "Deliver (i, Create i e2) \<notin> set (history k)"
+      using f4 f3 f2 f1 by (metis (full_types) added_files_Deliver_Create_collapse added_files_Deliver_Store_same_collapse empty_set fst_conv list.set_intros(1) network_axioms)
+    { assume "added_files [Deliver (i, Store e1 mo i)] e2 = []"
+      then have "Deliver (i, Append i e2) \<notin> set (history k)"
+        using f4 f3 f2 f1 by (metis (full_types) added_files_Deliver_Append_same_collapse empty_set fst_conv list.set_intros(1) network_axioms)
+      then have "e1 = e2"
+        using f8 f7 f6 f5 f1 by (metis (no_types) \<open>pre prefix of k\<close> added_files_Deliver_Store_diff_collapse empty_set list.set_intros(1) prefix_elem_to_carriers) }
+    then have "(i, Store e2 mo i) \<in> set (node_deliver_messages xs)"
+      by (metis (no_types) added_files_Deliver_Store_diff_collapse assms(3))
+    then show "\<not> network history f \<or> Deliver (i, Store e2 mo i) \<in> set (history j)"
+      by (meson assms(2) network.prefix_msg_in_history)
   qed 
-  	then have f2: "Deliver (i, Store e2 mo i) \<in> set (history j)"
-  		using network_axioms by blast
-  	obtain nn :: "'a \<times> ('a, 'b) operation \<Rightarrow> nat" where
-  		f3: "\<And>p n. Deliver p \<notin> set (history n) \<or> Broadcast p \<in> set (history (nn p))"
-  		by (metis delivery_has_a_cause)
-  	then have f4: "Broadcast (i, Store e2 mo i) \<in> set (history (nn (i, Store e2 mo i)))"
-  		using f2 by blast
-		have "\<And>p. Deliver p \<notin> set pre \<or> Broadcast p \<in> set (history (nn p))"
-			using f3 f1 by blast
-		then show ?thesis
-			using f4 by (metis (no_types) A fst_conv msg_id_unique)
-	qed
-  		
-  	moreover have "Deliver(i, Store e1 mo i) \<in> set (history j)"
+    then have f2: "Deliver (i, Store e2 mo i) \<in> set (history j)"
+      using network_axioms by blast
+    obtain nn :: "'a \<times> ('a, 'b) operation \<Rightarrow> nat" where
+      f3: "\<And>p n. Deliver p \<notin> set (history n) \<or> Broadcast p \<in> set (history (nn p))"
+      by (metis delivery_has_a_cause)
+    then have f4: "Broadcast (i, Store e2 mo i) \<in> set (history (nn (i, Store e2 mo i)))"
+      using f2 by blast
+    have "\<And>p. Deliver p \<notin> set pre \<or> Broadcast p \<in> set (history (nn p))"
+      using f3 f1 by blast
+    then show ?thesis
+      using f4 by (metis (no_types) A fst_conv msg_id_unique)
+  qed      
+    moreover have "Deliver(i, Store e1 mo i) \<in> set (history j)"
     using assms(2) assms(3) prefix_msg_in_history by blast 
   ultimately show ?thesis
-  	by (metis (no_types, lifting) delivery_has_a_cause fst_conv network.msg_id_unique network_axioms operation.inject(5) prefix_elem_to_carriers prefix_of_appendD prod.inject)
+    by (metis (no_types, lifting) delivery_has_a_cause fst_conv network.msg_id_unique network_axioms operation.inject(5) prefix_elem_to_carriers prefix_of_appendD prod.inject)
 qed
 
-lemma (in imap) add_rem_ids_imply_messages_same:
+lemma (in imap) create_delete_ids_imply_messages_same:
   assumes "i \<in> is"
     and "xs prefix of j"
-    and "(i, Add i e1) \<in> set (node_deliver_messages xs)" and "(ir, Rem is e2) \<in> set (node_deliver_messages xs)"
+    and "(i, Create i e1) \<in> set (node_deliver_messages xs)" 
+    and "(ir, Delete is e2) \<in> set (node_deliver_messages xs)"
   shows "e1 = e2"
 proof -
-  obtain pre k where P: "pre@[Broadcast (ir, Rem is e2)] prefix of k"
+  obtain pre k where P: "pre@[Broadcast (ir, Delete is e2)] prefix of k"
     using assms delivery_has_a_cause events_before_exist prefix_msg_in_history by blast
-  moreover hence A: "Deliver (i, Add i e2) \<in> set pre \<or> Deliver (i, Append i e2) \<in> set pre \<or> (\<exists> mo . Deliver (i, Expunge e2 mo i) \<in> set pre) \<or> (\<exists> mo . Deliver (i, Store e2 mo i) \<in> set pre)"
-    using Broadcast_Deliver_prefix_closed assms(1) ids_are_unique by blast
-    	
-  hence "Deliver (i, Add i e2) \<in> set pre" using assms ids_are_unique P
+  moreover hence A: "Deliver (i, Create i e2) \<in> set pre \<or> Deliver (i, Append i e2) \<in> set pre \<or> (\<exists> mo . Deliver (i, Expunge e2 mo i) \<in> set pre) \<or> (\<exists> mo . Deliver (i, Store e2 mo i) \<in> set pre)"
+    using Broadcast_Deliver_prefix_closed assms(1) ids_are_unique by blast      
+  hence "Deliver (i, Create i e2) \<in> set pre" using assms ids_are_unique P
 proof -
-  	obtain aa :: 'a and aaa :: 'a where
-  		f1: "(Deliver (i, Append i e2) \<in> set pre \<or> (\<exists>a. Deliver (i, Expunge e2 a i) \<in> set pre) \<or> (\<exists>a. Deliver (i, Store e2 a i) \<in> set pre)) = (Deliver (i, Append i e2) \<in> set pre \<or> Deliver (i, Expunge e2 aaa i) \<in> set pre \<or> Deliver (i, Store e2 aa i) \<in> set pre)"
-  		by blast
-  	have f2: "\<forall>p n pa na. Broadcast p \<notin> set (history n) \<or> Broadcast pa \<notin> set (history na) \<or> fst p \<noteq> fst pa \<or> n = na \<and> p = pa"
-  		using msg_id_unique by presburger
-  	obtain nn :: "'a \<times> ('a, 'b) operation \<Rightarrow> nat" where
-  		f3: "\<forall>p n. Deliver p \<notin> set (history n) \<or> Broadcast p \<in> set (history (nn p))"
-  		by (metis (no_types) delivery_has_a_cause)
-		then have f4: "Broadcast (i, Add i e2) \<in> set (history (nn (i, Add i e2)))"
-			using assms prefix_msg_in_history P A
-		proof -
-			obtain aab :: 'a and aac :: 'a where
-    x1: "Deliver (i, Add i e2) \<in> set pre \<or> Deliver (i, Append i e2) \<in> set pre \<or> Deliver (i, Expunge e2 aac i) \<in> set pre \<or> Deliver (i, Store e2 aab i) \<in> set pre"
-    using A by blast
-  have x2: "\<forall>f fa p n pa na. \<not> network f fa \<or> Broadcast (p::'a \<times> ('a, 'b) operation) \<notin> set (f n) \<or> Broadcast pa \<notin> set (f na) \<or> (fa p::'a) \<noteq> fa pa \<or> n = na \<and> p = pa"
-    by (meson network.msg_id_unique)
-  have x3: "Broadcast (i, Add i e1) \<in> set (history (nn (i, Add i e1)))"
-    using assms(2) assms(3) f3 prefix_msg_in_history by blast
-  then have x4: "Deliver (i, Store e2 aab i) \<notin> set (history k)"
-    using x2 by (metis (full_types) added_files_Deliver_Add_collapse added_files_Deliver_Store_same_collapse empty_iff empty_set f3 fst_conv list.set_intros(1) network_axioms)
-  have x5: "Deliver (i, Append i e2) \<notin> set (history k)"
-    using x3 f2 by (metis (full_types) added_files_Deliver_Add_collapse added_files_Deliver_Append_same_collapse empty_iff empty_set f3 fst_conv list.set_intros(1))
-  have "Deliver (i, Expunge e2 aac i) \<notin> set (history k)"
-    using x3 f2 by (metis (no_types) f3 fst_conv operation.distinct(5) prod.inject)
-  then show ?thesis
-    using x5 x4 x1 calculation f3 prefix_elem_to_carriers by blast
-qed 
-		have f5: "\<forall>es n e. \<not> es prefix of n \<or> e \<notin> set es \<or> e \<in> set (history n)"
-			using prefix_elem_to_carriers by blast
-		then have f6: "Deliver (i, Append i e2) \<in> set pre \<longrightarrow> nn (i, Append i e2) = nn (i, Add i e2) \<and> (i, Append i e2) = (i, Add i e2)"
-			using f4 f3 f2	by (metis calculation fst_conv node_histories.prefix_of_appendD node_histories_axioms) 
-
-		have f7: "Deliver (i, Expunge e2 aaa i) \<in> set pre \<longrightarrow> nn (i, Expunge e2 aaa i) = nn (i, Add i e2) \<and> (i, Expunge e2 aaa i) = (i, Add i e2)"
-			using f5 f4 f3 f2 by (metis calculation fst_conv node_histories.prefix_of_appendD node_histories_axioms)
-		have "Deliver (i, Store e2 aa i) \<in> set pre \<longrightarrow> Deliver (i, Add i e2) \<in> set pre"
-			using f5 f4 f3 f2 by (metis calculation fst_conv node_histories.prefix_of_appendD node_histories_axioms)
-		then show ?thesis
-			using f7 f6 f1 A by blast
-	qed
-  		
-  moreover have "Deliver (i, Add i e1) \<in> set (history j)"
+    obtain aa :: 'a and aaa :: 'a where
+      f1: "(Deliver (i, Append i e2) \<in> set pre \<or> (\<exists>a. Deliver (i, Expunge e2 a i) \<in> set pre) \<or> (\<exists>a. Deliver (i, Store e2 a i) \<in> set pre)) = (Deliver (i, Append i e2) \<in> set pre \<or> Deliver (i, Expunge e2 aaa i) \<in> set pre \<or> Deliver (i, Store e2 aa i) \<in> set pre)"
+      by blast
+    have f2: "\<forall>p n pa na. Broadcast p \<notin> set (history n) \<or> Broadcast pa \<notin> set (history na) \<or> fst p \<noteq> fst pa \<or> n = na \<and> p = pa"
+      using msg_id_unique by presburger
+    obtain nn :: "'a \<times> ('a, 'b) operation \<Rightarrow> nat" where
+      f3: "\<forall>p n. Deliver p \<notin> set (history n) \<or> Broadcast p \<in> set (history (nn p))"
+      by (metis (no_types) delivery_has_a_cause)
+    then have f4: "Broadcast (i, Create i e2) \<in> set (history (nn (i, Create i e2)))"
+      using assms prefix_msg_in_history P A
+    proof -
+      obtain aab :: 'a and aac :: 'a where
+        x1: "Deliver (i, Create i e2) \<in> set pre \<or> Deliver (i, Append i e2) \<in> set pre \<or> Deliver (i, Expunge e2 aac i) \<in> set pre \<or> Deliver (i, Store e2 aab i) \<in> set pre"
+        using A by blast
+      have x2: "\<forall>f fa p n pa na. \<not> network f fa \<or> Broadcast (p::'a \<times> ('a, 'b) operation) \<notin> set (f n) \<or> Broadcast pa \<notin> set (f na) \<or> (fa p::'a) \<noteq> fa pa \<or> n = na \<and> p = pa"
+        by (meson network.msg_id_unique)
+      have x3: "Broadcast (i, Create i e1) \<in> set (history (nn (i, Create i e1)))"
+        using assms(2) assms(3) f3 prefix_msg_in_history by blast
+      then have x4: "Deliver (i, Store e2 aab i) \<notin> set (history k)"
+        using x2 by (metis (full_types) added_files_Deliver_Create_collapse added_files_Deliver_Store_same_collapse empty_iff empty_set f3 fst_conv list.set_intros(1) network_axioms)
+      have x5: "Deliver (i, Append i e2) \<notin> set (history k)"
+        using x3 f2 by (metis (full_types) added_files_Deliver_Create_collapse added_files_Deliver_Append_same_collapse empty_iff empty_set f3 fst_conv list.set_intros(1))
+      have "Deliver (i, Expunge e2 aac i) \<notin> set (history k)"
+        using x3 f2 by (metis (no_types) f3 fst_conv operation.distinct(5) prod.inject)
+      then show ?thesis
+        using x5 x4 x1 calculation f3 prefix_elem_to_carriers by blast
+    qed 
+    have f5: "\<forall>es n e. \<not> es prefix of n \<or> e \<notin> set es \<or> e \<in> set (history n)"
+      using prefix_elem_to_carriers by blast
+    then have f6: "Deliver (i, Append i e2) \<in> set pre \<longrightarrow> nn (i, Append i e2) = nn (i, Create i e2) \<and> (i, Append i e2) = (i, Create i e2)"
+      using f4 f3 f2  by (metis calculation fst_conv node_histories.prefix_of_appendD node_histories_axioms)
+    have f7: "Deliver (i, Expunge e2 aaa i) \<in> set pre \<longrightarrow> nn (i, Expunge e2 aaa i) = nn (i, Create i e2) \<and> (i, Expunge e2 aaa i) = (i, Create i e2)"
+      using f5 f4 f3 f2 by (metis calculation fst_conv node_histories.prefix_of_appendD node_histories_axioms)
+    have "Deliver (i, Store e2 aa i) \<in> set pre \<longrightarrow> Deliver (i, Create i e2) \<in> set pre"
+      using f5 f4 f3 f2 by (metis calculation fst_conv node_histories.prefix_of_appendD node_histories_axioms)
+    then show ?thesis
+      using f7 f6 f1 A by blast
+  qed      
+  moreover have "Deliver (i, Create i e1) \<in> set (history j)"
     using assms(2) assms(3) prefix_msg_in_history by blast
   ultimately show ?thesis
     by (metis fst_conv msg_id_unique network.delivery_has_a_cause network_axioms operation.inject(1)
         prefix_elem_to_carriers prefix_of_appendD prod.inject)
 qed
-	
-lemma (in imap) append_rem_ids_imply_messages_same:
+  
+lemma (in imap) append_delete_ids_imply_messages_same:
   assumes "i \<in> is"
     and "xs prefix of j"
-    and "(i, Append i e1) \<in> set (node_deliver_messages xs)" and "(ir, Rem is e2) \<in> set (node_deliver_messages xs)"
+    and "(i, Append i e1) \<in> set (node_deliver_messages xs)" 
+    and "(ir, Delete is e2) \<in> set (node_deliver_messages xs)"
   shows "e1 = e2"
 proof -
-  obtain pre k where P: "pre@[Broadcast (ir, Rem is e2)] prefix of k"
-    using assms delivery_has_a_cause events_before_exist prefix_msg_in_history by blast
-  
-   moreover hence A: "Deliver (i, Add i e2) \<in> set pre \<or> Deliver (i, Append i e2) \<in> set pre \<or> (\<exists> mo . Deliver (i, Expunge e2 mo i) \<in> set pre) \<or> (\<exists> mo . Deliver (i, Store e2 mo i) \<in> set pre)"
+  obtain pre k where P: "pre@[Broadcast (ir, Delete is e2)] prefix of k"
+    using assms delivery_has_a_cause events_before_exist prefix_msg_in_history by blast  
+   moreover hence A: "Deliver (i, Create i e2) \<in> set pre \<or> Deliver (i, Append i e2) \<in> set pre \<or> (\<exists> mo . Deliver (i, Expunge e2 mo i) \<in> set pre) \<or> (\<exists> mo . Deliver (i, Store e2 mo i) \<in> set pre)"
     using Broadcast_Deliver_prefix_closed assms(1)
-    by (meson imap.Broadcast_Deliver_prefix_closed imap_axioms)
-    	
+    by (meson imap.Broadcast_Deliver_prefix_closed imap_axioms)      
   hence "Deliver (i, Append i e2) \<in> set pre" using assms ids_are_unique 
-		proof -
-			have f1: "\<forall>f fa p n pa na. \<not> network f fa \<or> Broadcast (p::'a \<times> ('a, 'b) operation) \<notin> set (f n) \<or> Broadcast pa \<notin> set (f na) \<or> (fa p::'a) \<noteq> fa pa \<or> n = na \<and> p = pa"
-				by (meson network.msg_id_unique)
-			obtain nn :: "'a \<times> ('a, 'b) operation \<Rightarrow> nat" where
-				f2: "\<forall>p n. Deliver p \<notin> set (history n) \<or> Broadcast p \<in> set (history (nn p))"
-				by (metis (no_types) delivery_has_a_cause)
-			then have f3: "Broadcast (i, Append i e1) \<in> set (history (nn (i, Append i e1)))"
-				using assms(2) assms(3) prefix_msg_in_history by blast
-			obtain aa :: 'a and aaa :: 'a where
-				f4: "(Deliver (i, Add i e2) \<in> set pre \<or> (\<exists>a. Deliver (i, Expunge e2 a i) \<in> set pre) \<or> (\<exists>a. Deliver (i, Store e2 a i) \<in> set pre)) = (Deliver (i, Add i e2) \<in> set pre \<or> Deliver (i, Expunge e2 aaa i) \<in> set pre \<or> Deliver (i, Store e2 aa i) \<in> set pre)"
-				by blast
-			have f5: "\<forall>a. (a::'a) \<notin> {}"
-				by (meson empty_iff)
-			have f6: "\<forall>e. e \<notin> set pre \<or> e \<in> set (history k)"
-				by (meson calculation node_histories.prefix_of_appendD node_histories_axioms prefix_to_carriers subset_iff)
-			then have "Deliver (i, Store e2 aa i) \<in> set pre \<longrightarrow> Broadcast (i, Store e2 aa i) \<in> set (history (nn (i, Store e2 aa i)))"
-				using f2 by blast
-			then have f7: "Deliver (i, Store e2 aa i) \<in> set pre \<longrightarrow> nn (i, Store e2 aa i) = nn (i, Append i e1) \<and> (i, Store e2 aa i) = (i, Append i e1)"
-				using f3 f1 by (metis fst_conv network_axioms)
-			have f8: "Deliver (i, Add i e2) \<notin> set pre"
-				using f6 f5 f3 f2 f1 by (metis (no_types) added_files_Deliver_Add_collapse added_files_Deliver_Append_same_collapse empty_set fst_conv list.set_intros(1) network_axioms)
-			have "Deliver (i, Expunge e2 aaa i) \<notin> set pre"
-				using f6 f5 f3 f2 f1 by (metis (no_types) added_files_Deliver_Append_same_collapse added_files_Deliver_Expunge_collapse empty_set fst_conv list.set_intros(1) network_axioms)
-			then show ?thesis
-				using f8 f7 f4 A by blast
-		qed      
-  	moreover have "Deliver (i, Append i e1) \<in> set (history j)"
+    proof -
+      have f1: "\<forall>f fa p n pa na. \<not> network f fa \<or> Broadcast (p::'a \<times> ('a, 'b) operation) \<notin> set (f n) \<or> Broadcast pa \<notin> set (f na) \<or> (fa p::'a) \<noteq> fa pa \<or> n = na \<and> p = pa"
+        by (meson network.msg_id_unique)
+      obtain nn :: "'a \<times> ('a, 'b) operation \<Rightarrow> nat" where
+        f2: "\<forall>p n. Deliver p \<notin> set (history n) \<or> Broadcast p \<in> set (history (nn p))"
+        by (metis (no_types) delivery_has_a_cause)
+      then have f3: "Broadcast (i, Append i e1) \<in> set (history (nn (i, Append i e1)))"
+        using assms(2) assms(3) prefix_msg_in_history by blast
+      obtain aa :: 'a and aaa :: 'a where
+        f4: "(Deliver (i, Create i e2) \<in> set pre \<or> (\<exists>a. Deliver (i, Expunge e2 a i) \<in> set pre) \<or> (\<exists>a. Deliver (i, Store e2 a i) \<in> set pre)) = (Deliver (i, Create i e2) \<in> set pre \<or> Deliver (i, Expunge e2 aaa i) \<in> set pre \<or> Deliver (i, Store e2 aa i) \<in> set pre)"
+        by blast
+      have f5: "\<forall>a. (a::'a) \<notin> {}"
+        by (meson empty_iff)
+      have f6: "\<forall>e. e \<notin> set pre \<or> e \<in> set (history k)"
+        by (meson calculation node_histories.prefix_of_appendD node_histories_axioms prefix_to_carriers subset_iff)
+      then have "Deliver (i, Store e2 aa i) \<in> set pre \<longrightarrow> Broadcast (i, Store e2 aa i) \<in> set (history (nn (i, Store e2 aa i)))"
+        using f2 by blast
+      then have f7: "Deliver (i, Store e2 aa i) \<in> set pre \<longrightarrow> nn (i, Store e2 aa i) = nn (i, Append i e1) \<and> (i, Store e2 aa i) = (i, Append i e1)"
+        using f3 f1 by (metis fst_conv network_axioms)
+      have f8: "Deliver (i, Create i e2) \<notin> set pre"
+        using f6 f5 f3 f2 f1 by (metis (no_types) added_files_Deliver_Create_collapse added_files_Deliver_Append_same_collapse empty_set fst_conv list.set_intros(1) network_axioms)
+      have "Deliver (i, Expunge e2 aaa i) \<notin> set pre"
+        using f6 f5 f3 f2 f1 by (metis (no_types) added_files_Deliver_Append_same_collapse added_files_Deliver_Expunge_collapse empty_set fst_conv list.set_intros(1) network_axioms)
+      then show ?thesis
+        using f8 f7 f4 A by blast
+    qed      
+    moreover have "Deliver (i, Append i e1) \<in> set (history j)"
     using assms(2) assms(3) prefix_msg_in_history by blast
   ultimately show ?thesis
     by (metis (no_types, lifting) fst_conv network.delivery_has_a_cause network.msg_id_unique network_axioms operation.inject(3) prefix_elem_to_carriers prefix_of_appendD prod.inject)
@@ -618,162 +619,158 @@ qed
 lemma (in imap) append_expunge_ids_imply_messages_same:
   assumes "i = mo"
     and "xs prefix of j"
-    and "(i, Append i e1) \<in> set (node_deliver_messages xs)" and "(r, Expunge e2 mo r) \<in> set (node_deliver_messages xs)"
+    and "(i, Append i e1) \<in> set (node_deliver_messages xs)" 
+    and "(r, Expunge e2 mo r) \<in> set (node_deliver_messages xs)"
   shows "e1 = e2"
 proof -
   obtain pre k where "pre@[Broadcast (r, Expunge e2 mo r)] prefix of k"
-    using assms delivery_has_a_cause events_before_exist prefix_msg_in_history by blast
-  
+    using assms delivery_has_a_cause events_before_exist prefix_msg_in_history by blast  
    moreover hence "Deliver (mo, Append mo e2) \<in> set pre \<or> (\<exists> mo2 . Deliver (mo, Store e2 mo2 mo) \<in> set pre)"
     using Broadcast_Expunge_Deliver_prefix_closed assms(1)
-    by (meson imap.Broadcast_Deliver_prefix_closed imap_axioms)
-    	
+    by (meson imap.Broadcast_Deliver_prefix_closed imap_axioms)      
   hence "Deliver (i, Append i e2) \<in> set pre" using assms ids_are_unique
   proof -
-  	have f1: "Store e2 v0_0 mo \<noteq> Append i e1"
+    have f1: "Store e2 X mo \<noteq> Append i e1"
     by blast
   have f2: "Deliver (i, Append i e1) \<in> set (history j)"
     using \<open>(i, Append i e1) \<in> set (node_deliver_messages xs)\<close> \<open>xs prefix of j\<close> prefix_msg_in_history by blast
   obtain aa :: 'a where
     f3: "Deliver (mo, Append mo e2) \<in> set pre \<or> Deliver (mo, Store e2 aa mo) \<in> set pre"
     using \<open>Deliver (mo, Append mo e2) \<in> set pre \<or> (\<exists>mo2. Deliver (mo, Store e2 mo2 mo) \<in> set pre)\<close> by blast
-    	have "pre prefix of k"
-    		using calculation by blast
-    	then have "Deliver (mo, Store e2 aa mo) \<notin> set pre"
-    		using f2 f1  Pair_inject assms delivery_has_a_cause fst_conv msg_id_unique prefix_elem_to_carriers
-    		by (metis operation.distinct(17)) 
-    	then have "Deliver (mo, Append mo e2) \<in> set pre"
-    		using f3 by meson
-    	then show ?thesis
-    		by (simp add: \<open>i = mo\<close>)
+      have "pre prefix of k"
+        using calculation by blast
+      then have "Deliver (mo, Store e2 aa mo) \<notin> set pre"
+        using f2 f1  Pair_inject assms delivery_has_a_cause fst_conv msg_id_unique prefix_elem_to_carriers
+        by (metis operation.distinct(17)) 
+      then have "Deliver (mo, Append mo e2) \<in> set pre"
+        using f3 by meson
+      then show ?thesis
+        by (simp add: \<open>i = mo\<close>)
     qed       
-  	moreover have "Deliver (i, Append i e1) \<in> set (history j)"
+    moreover have "Deliver (i, Append i e1) \<in> set (history j)"
     using assms(2) assms(3) prefix_msg_in_history by blast
   ultimately show ?thesis
     by (metis (no_types, lifting) fst_conv network.delivery_has_a_cause network.msg_id_unique network_axioms operation.inject(3) prefix_elem_to_carriers prefix_of_appendD prod.inject)
 qed
-	
-	
+ 
 lemma (in imap) append_store_ids_imply_messages_same:
   assumes "i = mo"
     and "xs prefix of j"
-    and "(i, Append i e1) \<in> set (node_deliver_messages xs)" and "(r, Store e2 mo r) \<in> set (node_deliver_messages xs)"
+    and "(i, Append i e1) \<in> set (node_deliver_messages xs)" 
+    and "(r, Store e2 mo r) \<in> set (node_deliver_messages xs)"
   shows "e1 = e2"
 proof -
   obtain pre k where P: "pre@[Broadcast (r, Store e2 mo r)] prefix of k"
-    using assms delivery_has_a_cause events_before_exist prefix_msg_in_history by blast
-  
-   moreover hence A: "Deliver (mo, Append mo e2) \<in> set pre \<or> (\<exists> mo2 . Deliver (mo, Store e2 mo2 mo) \<in> set pre)"
+    using assms delivery_has_a_cause events_before_exist prefix_msg_in_history by blast  
+  moreover hence A: "Deliver (mo, Append mo e2) \<in> set pre \<or> (\<exists> mo2 . Deliver (mo, Store e2 mo2 mo) \<in> set pre)"
     using Broadcast_Store_Deliver_prefix_closed assms(1)
-    by (meson imap.Broadcast_Deliver_prefix_closed imap_axioms)
-    	
+    by (meson imap.Broadcast_Deliver_prefix_closed imap_axioms)      
   have "Deliver (i, Append i e2) \<in> set pre" using assms ids_are_unique P A
   proof -
-  	have f1: "Deliver (i, Append i e1) \<in> set (history j)"
-  		using assms(2) assms(3) prefix_msg_in_history by blast
-  	obtain aa :: 'a where
-  		f2: "Deliver (mo, Append mo e2) \<in> set pre \<or> Deliver (mo, Store e2 aa mo) \<in> set pre"
-  		using A by blast
-  	have f3: "pre prefix of k"
-  		using calculation by blast
-  	have f4: "fst (mo, Store e2 aa mo) = fst (i, Append i e1)"
-  		using assms(1) by auto
-  	have "v2_1 (mo, Store e2 aa mo) \<noteq> (v2_1 (i, Append i e1)::nat) \<or> (mo, Store e2 aa mo) \<noteq> (i, Append i e1)"
-  		by force
-  	then have "Deliver (mo, Store e2 aa mo) \<notin> set (history k)"
-  		using f4 f1 by (metis (no_types) delivery_has_a_cause network.msg_id_unique network_axioms)
-  	then show ?thesis
-  		using f3 f2 assms(1) prefix_elem_to_carriers by blast
+    have f1: "Deliver (i, Append i e1) \<in> set (history j)"
+      using assms(2) assms(3) prefix_msg_in_history by blast
+    obtain aa :: 'a where
+      f2: "Deliver (mo, Append mo e2) \<in> set pre \<or> Deliver (mo, Store e2 aa mo) \<in> set pre"
+      using A by blast
+    have f3: "pre prefix of k"
+      using calculation by blast
+    have f4: "fst (mo, Store e2 aa mo) = fst (i, Append i e1)"
+      using assms(1) by auto
+    have "v2_1 (mo, Store e2 aa mo) \<noteq> (v2_1 (i, Append i e1)::nat) \<or> (mo, Store e2 aa mo) \<noteq> (i, Append i e1)"
+      by force
+    then have "Deliver (mo, Store e2 aa mo) \<notin> set (history k)"
+      using f4 f1 by (metis (no_types) delivery_has_a_cause network.msg_id_unique network_axioms)
+    then show ?thesis
+      using f3 f2 assms(1) prefix_elem_to_carriers by blast
   qed      
-  	moreover have "Deliver (i, Append i e1) \<in> set (history j)"
+    moreover have "Deliver (i, Append i e1) \<in> set (history j)"
     using assms(2) assms(3) prefix_msg_in_history by blast
   ultimately show ?thesis
     by (metis (no_types, lifting) fst_conv network.delivery_has_a_cause network.msg_id_unique network_axioms operation.inject(3) prefix_elem_to_carriers prefix_of_appendD prod.inject)
 qed
-	
+  
 lemma (in imap) expunge_store_ids_imply_messages_same:
-    assumes "xs prefix of j"
-    and "(i, Store e1 mo i) \<in> set (node_deliver_messages xs)" and "(r, Expunge e2 i r) \<in> set (node_deliver_messages xs)"
+  assumes "xs prefix of j"
+    and "(i, Store e1 mo i) \<in> set (node_deliver_messages xs)" 
+    and "(r, Expunge e2 i r) \<in> set (node_deliver_messages xs)"
   shows "e1 = e2"
 proof -
   obtain pre k where P: "pre@[Broadcast (r, Expunge e2 i r)] prefix of k"
-    using assms delivery_has_a_cause events_before_exist prefix_msg_in_history by blast
-  
-   moreover hence A: "Deliver (i, Append i e2) \<in> set pre \<or> (\<exists> mo2 . Deliver (i, Store e2 mo2 i) \<in> set pre)"
-    using Broadcast_Expunge_Deliver_prefix_closed assms(1) by blast
-    	
+    using assms delivery_has_a_cause events_before_exist prefix_msg_in_history by blast  
+  moreover hence A: "Deliver (i, Append i e2) \<in> set pre \<or> (\<exists> mo2 . Deliver (i, Store e2 mo2 i) \<in> set pre)"
+    using Broadcast_Expunge_Deliver_prefix_closed assms(1) by blast      
   have B: "Deliver (i, Store e2 mo i) \<in> set pre" using assms ids_are_unique A P
   proof -
-  	obtain nn :: "'a \<times> ('a, 'b) operation \<Rightarrow> nat" where
-  		f1: "\<And>p n. Deliver p \<notin> set (history n) \<or> Broadcast p \<in> set (history (nn p))"
-  		by (metis (no_types) delivery_has_a_cause)
-  	then have "Broadcast (i, Store e2 mo i) \<in> set (history (nn (i, Store e2 mo i)))"
-  		using assms(1) assms(2) prefix_msg_in_history
-proof -
-  have x1: "Broadcast (i, Store e1 mo i) \<in> set (history (nn (i, Store e1 mo i)))"
-    using assms(1) assms(2) f1 prefix_msg_in_history by blast
-  have x2: "\<forall>b a aa ba ab ac. (Store (b::'b) (a::'a) aa = Store ba ab ac) = (b = ba \<and> a = ab \<and> aa = ac)"
-    by blast
-  have x3: "\<forall>a z aa za. (a::'a, z::('a, 'b) operation) \<noteq> (aa, za) \<or> a = aa \<and> z = za"
-    by blast
-  have x4: "(\<forall>a z aa za. (a::'a, z::('a, 'b) operation) \<noteq> (aa, za) \<or> a = aa \<and> z = za) = (\<forall>a z aa za. (a::'a, z::('a, 'b) operation) \<noteq> (aa, za) \<or> a = aa \<and> z = za)"
-    by meson
-    	have x5: "\<forall>p n pa na. Broadcast p \<notin> set (history n) \<or> Broadcast pa \<notin> set (history na) \<or> fst p \<noteq> fst pa \<or> n = na \<and> p = pa"
-    		using msg_id_unique by blast
-    	then obtain aa :: 'a where
-    		"Deliver (i, Store e2 aa i) \<in> set (history k)"
-    using x3 x1 by (metis A calculation f1 fst_conv node_histories.prefix_of_appendD node_histories_axioms operation.distinct(17) prefix_elem_to_carriers)
-  then have "e2 = e1 \<and> aa = mo"
-    using x5 x4 x3 x2 x1 by (metis (no_types) f1 fst_conv)
-  then show ?thesis
-    using x1 by force
-qed  
-  	then show ?thesis
-  		using f1 by (metis (no_types) A calculation fst_conv msg_id_unique prefix_elem_to_carriers prefix_of_appendD)
+    obtain nn :: "'a \<times> ('a, 'b) operation \<Rightarrow> nat" where
+      f1: "\<And>p n. Deliver p \<notin> set (history n) \<or> Broadcast p \<in> set (history (nn p))"
+      by (metis (no_types) delivery_has_a_cause)
+    then have "Broadcast (i, Store e2 mo i) \<in> set (history (nn (i, Store e2 mo i)))"
+      using assms(1) assms(2) prefix_msg_in_history
+  proof -
+    have x1: "Broadcast (i, Store e1 mo i) \<in> set (history (nn (i, Store e1 mo i)))"
+      using assms(1) assms(2) f1 prefix_msg_in_history by blast
+    have x2: "\<forall>b a aa ba ab ac. (Store (b::'b) (a::'a) aa = Store ba ab ac) = (b = ba \<and> a = ab \<and> aa = ac)"
+      by blast
+    have x3: "\<forall>a z aa za. (a::'a, z::('a, 'b) operation) \<noteq> (aa, za) \<or> a = aa \<and> z = za"
+      by blast
+    have x4: "(\<forall>a z aa za. (a::'a, z::('a, 'b) operation) \<noteq> (aa, za) \<or> a = aa \<and> z = za) = (\<forall>a z aa za. (a::'a, z::('a, 'b) operation) \<noteq> (aa, za) \<or> a = aa \<and> z = za)"
+      by meson
+        have x5: "\<forall>p n pa na. Broadcast p \<notin> set (history n) \<or> Broadcast pa \<notin> set (history na) \<or> fst p \<noteq> fst pa \<or> n = na \<and> p = pa"
+          using msg_id_unique by blast
+        then obtain aa :: 'a where
+          "Deliver (i, Store e2 aa i) \<in> set (history k)"
+      using x3 x1 by (metis A calculation f1 fst_conv node_histories.prefix_of_appendD node_histories_axioms operation.distinct(17) prefix_elem_to_carriers)
+    then have "e2 = e1 \<and> aa = mo"
+      using x5 x4 x3 x2 x1 by (metis (no_types) f1 fst_conv)
+    then show ?thesis
+      using x1 by force
+    qed  
+      then show ?thesis
+        using f1 by (metis (no_types) A calculation fst_conv msg_id_unique prefix_elem_to_carriers prefix_of_appendD)
   qed 
-  	moreover have "Deliver (i, Store e1 mo i) \<in> set (history j)"
+  moreover have "Deliver (i, Store e1 mo i) \<in> set (history j)"
     using assms(1) assms(2) prefix_msg_in_history by auto
   ultimately show ?thesis using assms
-  	by (metis delivery_has_a_cause fst_conv msg_id_unique operation.inject(5) prefix_elem_to_carriers prefix_of_appendD prod.inject) 
-qed 
-	
+    by (metis delivery_has_a_cause fst_conv msg_id_unique operation.inject(5) prefix_elem_to_carriers prefix_of_appendD prod.inject) 
+qed
+  
 lemma (in imap) store_store_ids_imply_messages_same:
-    assumes "xs prefix of j"
-    and "(i, Store e1 mo i) \<in> set (node_deliver_messages xs)" and "(r, Store e2 i r) \<in> set (node_deliver_messages xs)"
+  assumes "xs prefix of j"
+    and "(i, Store e1 mo i) \<in> set (node_deliver_messages xs)" 
+    and "(r, Store e2 i r) \<in> set (node_deliver_messages xs)"
   shows "e1 = e2"
 proof -
   obtain pre k where P: "pre@[Broadcast (r, Store e2 i r)] prefix of k"
-    using assms delivery_has_a_cause events_before_exist prefix_msg_in_history by blast
-  
+    using assms delivery_has_a_cause events_before_exist prefix_msg_in_history by blast  
    moreover hence A: "Deliver (i, Append i e2) \<in> set pre \<or> (\<exists> mo2 . Deliver (i, Store e2 mo2 i) \<in> set pre)"
-   	 using Broadcast_Store_Deliver_prefix_closed assms(1) by blast
-   	 	 have B: "Deliver (i, Store e2 mo i) \<in> set pre" using assms ids_are_unique A P
-   	 	 proof -
-   	 	 	 obtain aa :: 'a where
-					f1: "Deliver (i, Append i e2) \<in> set pre \<or> Deliver (i, Store e2 aa i) \<in> set pre"
-					using A by blast
-				have f2: "\<forall>e. e \<notin> set pre \<or> e \<in> set (history k)"
-					by (metis (no_types) calculation node_histories.prefix_of_appendD node_histories_axioms prefix_to_carriers subset_iff)
-				have f3: "\<forall>f fa p n pa na. \<not> network f fa \<or> Broadcast (p::'a \<times> ('a, 'b) operation) \<notin> set (f n) \<or> Broadcast pa \<notin> set (f na) \<or> (fa p::'a) \<noteq> fa pa \<or> n = na \<and> p = pa"
-					by (meson network.msg_id_unique)
-				obtain nn :: "'a \<times> ('a, 'b) operation \<Rightarrow> nat" where
-					f4: "\<forall>p n. Deliver p \<notin> set (history n) \<or> Broadcast p \<in> set (history (nn p))"
-					by (metis delivery_has_a_cause)
-				then have f5: "Broadcast (i, Store e1 mo i) \<in> set (history (nn (i, Store e1 mo i)))"
-					using assms(1) assms(2) prefix_msg_in_history by blast
-				then have f6: "Deliver (i, Append i e2) \<notin> set pre"
-					using f4 f3 f2 by (metis (no_types) Pair_inject fst_conv network_axioms operation.distinct(17))
-				then have "Broadcast (i, Store e2 aa i) \<in> set (history (nn (i, Store e2 aa i)))"
-					using f4 f2 f1 by blast
-				then have "nn (i, Store e2 aa i) = nn (i, Store e1 mo i) \<and> (i, Store e2 aa i) = (i, Store e1 mo i)"
-					using f5 f3 by (metis fst_conv network_axioms)
-				then show ?thesis
-					using f6 f1 by force
-				qed
-  	moreover have "Deliver (i, Store e1 mo i) \<in> set (history j)"
+     using Broadcast_Store_Deliver_prefix_closed assms(1) by blast
+       have B: "Deliver (i, Store e2 mo i) \<in> set pre" using assms ids_are_unique A P
+       proof -
+         obtain aa :: 'a where
+          f1: "Deliver (i, Append i e2) \<in> set pre \<or> Deliver (i, Store e2 aa i) \<in> set pre"
+          using A by blast
+        have f2: "\<forall>e. e \<notin> set pre \<or> e \<in> set (history k)"
+          by (metis (no_types) calculation node_histories.prefix_of_appendD node_histories_axioms prefix_to_carriers subset_iff)
+        have f3: "\<forall>f fa p n pa na. \<not> network f fa \<or> Broadcast (p::'a \<times> ('a, 'b) operation) \<notin> set (f n) \<or> Broadcast pa \<notin> set (f na) \<or> (fa p::'a) \<noteq> fa pa \<or> n = na \<and> p = pa"
+          by (meson network.msg_id_unique)
+        obtain nn :: "'a \<times> ('a, 'b) operation \<Rightarrow> nat" where
+          f4: "\<forall>p n. Deliver p \<notin> set (history n) \<or> Broadcast p \<in> set (history (nn p))"
+          by (metis delivery_has_a_cause)
+        then have f5: "Broadcast (i, Store e1 mo i) \<in> set (history (nn (i, Store e1 mo i)))"
+          using assms(1) assms(2) prefix_msg_in_history by blast
+        then have f6: "Deliver (i, Append i e2) \<notin> set pre"
+          using f4 f3 f2 by (metis (no_types) Pair_inject fst_conv network_axioms operation.distinct(17))
+        then have "Broadcast (i, Store e2 aa i) \<in> set (history (nn (i, Store e2 aa i)))"
+          using f4 f2 f1 by blast
+        then have "nn (i, Store e2 aa i) = nn (i, Store e1 mo i) \<and> (i, Store e2 aa i) = (i, Store e1 mo i)"
+          using f5 f3 by (metis fst_conv network_axioms)
+        then show ?thesis
+          using f6 f1 by force
+        qed
+    moreover have "Deliver (i, Store e1 mo i) \<in> set (history j)"
     using assms(1) assms(2) prefix_msg_in_history by auto
   ultimately show ?thesis using assms
-  	by (metis delivery_has_a_cause fst_conv msg_id_unique operation.inject(5) prefix_elem_to_carriers prefix_of_appendD prod.inject) 
+    by (metis delivery_has_a_cause fst_conv msg_id_unique operation.inject(5) prefix_elem_to_carriers prefix_of_appendD prod.inject) 
 qed 
-	
+  
 end
