thys/IMAP-CRDT/IMAP-proof.thy
@@ -1,5 +1,7 @@
 section {* Convergence of the IMAP-CRDT *}
 
+text\<open>In this final section show that concurrent updates commute and thus Strong Eventual Convergence is achieved.\<close>
+
 theory
   "IMAP-proof"
 imports
@@ -9,64 +11,80 @@ imports
   "IMAP-proof-independent"
 begin
 
-corollary (in imap) concurrent_add_remove_independent:
-  assumes "\<not> hb (i, Add i e1) (ir, Rem is e2)" and "\<not> hb (ir, Rem is e2) (i, Add i e1)"
+corollary (in imap) concurrent_create_delete_independent:
+  assumes "\<not> hb (i, Create i e1) (ir, Delete is e2)" 
+    and "\<not> hb (ir, Delete is e2) (i, Create i e1)"
     and "xs prefix of j"
-    and "(i, Add i e1) \<in> set (node_deliver_messages xs)" and "(ir, Rem is e2) \<in> set (node_deliver_messages xs)"
+    and "(i, Create i e1) \<in> set (node_deliver_messages xs)" 
+    and "(ir, Delete is e2) \<in> set (node_deliver_messages xs)"
   shows "i \<notin> is"
-  using assms add_rem_ids_imply_messages_same concurrent_add_remove_independent_technical by fastforce
-  	
-corollary (in imap) concurrent_append_remove_independent:
-  assumes "\<not> hb (i, Append i e1) (ir, Rem is e2)" and "\<not> hb (ir, Rem is e2) (i, Append i e1)"
+  using assms create_delete_ids_imply_messages_same concurrent_create_delete_independent_technical by fastforce
+    
+corollary (in imap) concurrent_append_delete_independent:
+  assumes "\<not> hb (i, Append i e1) (ir, Delete is e2)" 
+    and "\<not> hb (ir, Delete is e2) (i, Append i e1)"
     and "xs prefix of j"
-    and "(i, Append i e1) \<in> set (node_deliver_messages xs)" and "(ir, Rem is e2) \<in> set (node_deliver_messages xs)"
+    and "(i, Append i e1) \<in> set (node_deliver_messages xs)" 
+    and "(ir, Delete is e2) \<in> set (node_deliver_messages xs)"
   shows "i \<notin> is"
-  using assms append_rem_ids_imply_messages_same concurrent_append_remove_independent_technical by fastforce
-  	
+  using assms append_delete_ids_imply_messages_same concurrent_append_delete_independent_technical by fastforce
+    
 corollary (in imap) concurrent_append_expunge_independent:
-  assumes "\<not> hb (i, Append i e1) (r, Expunge e2 mo r)" and "\<not> hb (r, Expunge e2 mo r) (i, Append i e1)"
+  assumes "\<not> hb (i, Append i e1) (r, Expunge e2 mo r)" 
+    and "\<not> hb (r, Expunge e2 mo r) (i, Append i e1)"
     and "xs prefix of j"
-    and "(i, Append i e1) \<in> set (node_deliver_messages xs)" and "(r, Expunge e2 mo r) \<in> set (node_deliver_messages xs)"
+    and "(i, Append i e1) \<in> set (node_deliver_messages xs)" 
+    and "(r, Expunge e2 mo r) \<in> set (node_deliver_messages xs)"
   shows "i \<noteq> mo"
   using assms append_expunge_ids_imply_messages_same concurrent_append_expunge_independent_technical by fastforce
-  	
+    
 corollary (in imap) concurrent_append_store_independent:
-  assumes "\<not> hb (i, Append i e1) (r, Store e2 mo r)" and "\<not> hb (r, Store e2 mo r) (i, Append i e1)"
+  assumes "\<not> hb (i, Append i e1) (r, Store e2 mo r)" 
+    and "\<not> hb (r, Store e2 mo r) (i, Append i e1)"
     and "xs prefix of j"
-    and "(i, Append i e1) \<in> set (node_deliver_messages xs)" and "(r, Store e2 mo r) \<in> set (node_deliver_messages xs)"
+    and "(i, Append i e1) \<in> set (node_deliver_messages xs)" 
+    and "(r, Store e2 mo r) \<in> set (node_deliver_messages xs)"
   shows "i \<noteq> mo"
   using assms append_store_ids_imply_messages_same concurrent_append_store_independent_technical by fastforce
     
-corollary (in imap) concurrent_expunge_remove_independent:
-  assumes "\<not> hb (i, Expunge e1 mo i) (ir, Rem is e2)" and "\<not> hb (ir, Rem is e2) (i, Expunge e1 mo i)"
+corollary (in imap) concurrent_expunge_delete_independent:
+  assumes "\<not> hb (i, Expunge e1 mo i) (ir, Delete is e2)" 
+    and "\<not> hb (ir, Delete is e2) (i, Expunge e1 mo i)"
     and "xs prefix of j"
-    and "(i, Expunge e1 mo i) \<in> set (node_deliver_messages xs)" and "(ir, Rem is e2) \<in> set (node_deliver_messages xs)"
+    and "(i, Expunge e1 mo i) \<in> set (node_deliver_messages xs)" 
+    and "(ir, Delete is e2) \<in> set (node_deliver_messages xs)"
   shows "i \<notin> is"
-  using assms expunge_rem_ids_imply_messages_same concurrent_expunge_remove_independent_technical by fastforce
-  	
-corollary (in imap) concurrent_store_remove_independent:
-  assumes "\<not> hb (i, Store e1 mo i) (ir, Rem is e2)" and "\<not> hb (ir, Rem is e2) (i, Store e1 mo i)"
+  using assms expunge_delete_ids_imply_messages_same concurrent_expunge_delete_independent_technical by fastforce
+    
+corollary (in imap) concurrent_store_delete_independent:
+  assumes "\<not> hb (i, Store e1 mo i) (ir, Delete is e2)" 
+    and "\<not> hb (ir, Delete is e2) (i, Store e1 mo i)"
     and "xs prefix of j"
-    and "(i, Store e1 mo i) \<in> set (node_deliver_messages xs)" and "(ir, Rem is e2) \<in> set (node_deliver_messages xs)"
+    and "(i, Store e1 mo i) \<in> set (node_deliver_messages xs)" 
+    and "(ir, Delete is e2) \<in> set (node_deliver_messages xs)"
   shows "i \<notin> is"
-  using assms store_rem_ids_imply_messages_same concurrent_store_remove_independent_technical by fastforce
-  	
+  using assms store_delete_ids_imply_messages_same concurrent_store_delete_independent_technical by fastforce
+    
 corollary (in imap) concurrent_store_expunge_independent:
-  assumes "\<not> hb (i, Store e1 mo i) (r, Expunge e2 mo2 r)" and "\<not> hb (r, Expunge e2 mo2 r) (i, Store e1 mo i)"
+  assumes "\<not> hb (i, Store e1 mo i) (r, Expunge e2 mo2 r)" 
+    and "\<not> hb (r, Expunge e2 mo2 r) (i, Store e1 mo i)"
     and "xs prefix of j"
-    and "(i, Store e1 mo i) \<in> set (node_deliver_messages xs)" and "(r, Expunge e2 mo2 r) \<in> set (node_deliver_messages xs)"
+    and "(i, Store e1 mo i) \<in> set (node_deliver_messages xs)" 
+    and "(r, Expunge e2 mo2 r) \<in> set (node_deliver_messages xs)"
   shows "i \<noteq> mo2 \<and> r \<noteq> mo"
   using assms expunge_store_ids_imply_messages_same concurrent_store_expunge_independent_technical2 concurrent_store_expunge_independent_technical 
   by metis
-  	
+    
 corollary (in imap) concurrent_store_store_independent:
-  assumes "\<not> hb (i, Store e1 mo i) (r, Store e2 mo2 r)" and "\<not> hb (r, Store e2 mo2 r) (i, Store e1 mo i)"
+  assumes "\<not> hb (i, Store e1 mo i) (r, Store e2 mo2 r)" 
+    and "\<not> hb (r, Store e2 mo2 r) (i, Store e1 mo i)"
     and "xs prefix of j"
-    and "(i, Store e1 mo i) \<in> set (node_deliver_messages xs)" and "(r, Store e2 mo2 r) \<in> set (node_deliver_messages xs)"
+    and "(i, Store e1 mo i) \<in> set (node_deliver_messages xs)" 
+    and "(r, Store e2 mo2 r) \<in> set (node_deliver_messages xs)"
   shows "i \<noteq> mo2 \<and> r \<noteq> mo"
   using assms store_store_ids_imply_messages_same concurrent_store_store_independent_technical 
-  	by metis
-  	
+    by metis
+    
 lemma (in imap) concurrent_operations_commute:
   assumes "xs prefix of i"
   shows "hb.concurrent_ops_commute (node_deliver_messages xs)"                     
@@ -76,30 +94,31 @@ proof -
            "(x, y) \<in> set (node_deliver_messages xs)"
            "hb.concurrent (a, b) (x, y)"
     hence "interp_msg (a, b) \<rhd> interp_msg (x, y) = interp_msg (x, y) \<rhd> interp_msg (a, b)" 
-      apply(unfold interp_msg_def, case_tac "b"; case_tac "y"; simp add: add_add_commute rem_rem_commute append_append_commute add_append_commute add_expunge_commute add_store_commute expunge_expunge_commute hb.concurrent_def)
-      using assms prefix_contains_msg apply (metis (full_types) add_id_valid add_rem_commute concurrent_add_remove_independent)
-      using assms prefix_contains_msg apply (metis (full_types) add_id_valid add_rem_commute concurrent_add_remove_independent)
-      using assms prefix_contains_msg apply (metis append_id_valid append_rem_ids_imply_messages_same concurrent_append_remove_independent_technical rem_append_commute)
-      using assms prefix_contains_msg apply (metis  concurrent_expunge_remove_independent expunge_id_valid imap.rem_expunge_commute imap_axioms)
-      using assms prefix_contains_msg apply (metis assms concurrent_store_remove_independent rem_store_commute store_id_valid)
-      using assms prefix_contains_msg apply (metis append_id_valid append_rem_ids_imply_messages_same concurrent_append_remove_independent_technical rem_append_commute)
+      apply(unfold interp_msg_def, case_tac "b"; case_tac "y"; simp add: create_create_commute delete_delete_commute append_append_commute create_append_commute create_expunge_commute create_store_commute expunge_expunge_commute hb.concurrent_def)
+      using assms prefix_contains_msg apply (metis (full_types) create_id_valid create_delete_commute concurrent_create_delete_independent)
+      using assms prefix_contains_msg apply (metis (full_types) create_id_valid create_delete_commute concurrent_create_delete_independent)
+      using assms prefix_contains_msg apply (metis append_id_valid append_delete_ids_imply_messages_same concurrent_append_delete_independent_technical delete_append_commute)
+      using assms prefix_contains_msg apply (metis  concurrent_expunge_delete_independent expunge_id_valid imap.delete_expunge_commute imap_axioms)
+      using assms prefix_contains_msg apply (metis assms concurrent_store_delete_independent delete_store_commute store_id_valid)
+      using assms prefix_contains_msg apply (metis append_id_valid append_delete_ids_imply_messages_same concurrent_append_delete_independent_technical delete_append_commute)
       using assms prefix_contains_msg apply (metis append_id_valid expunge_id_valid append_expunge_ids_imply_messages_same concurrent_append_expunge_independent_technical append_expunge_commute)
       using assms prefix_contains_msg apply (metis append_id_valid append_store_commute concurrent_append_store_independent store_id_valid)
-      using assms prefix_contains_msg	apply (metis concurrent_expunge_remove_independent expunge_id_valid rem_expunge_commute)
+      using assms prefix_contains_msg apply (metis concurrent_expunge_delete_independent expunge_id_valid delete_expunge_commute)
       using assms prefix_contains_msg apply (metis append_expunge_commute append_id_valid concurrent_append_expunge_independent expunge_id_valid)
       using assms prefix_contains_msg apply (metis expunge_id_valid expunge_store_commute imap.concurrent_store_expunge_independent imap_axioms store_id_valid)
-      using assms prefix_contains_msg apply (metis assms concurrent_store_remove_independent prefix_contains_msg rem_store_commute store_id_valid)
+      using assms prefix_contains_msg apply (metis assms concurrent_store_delete_independent prefix_contains_msg delete_store_commute store_id_valid)
       using assms prefix_contains_msg apply (metis append_id_valid append_store_commute imap.concurrent_append_store_independent imap_axioms store_id_valid)
       using assms prefix_contains_msg apply (metis expunge_id_valid expunge_store_commute imap.concurrent_store_expunge_independent imap_axioms store_id_valid)
-			using assms prefix_contains_msg	by (metis concurrent_store_store_independent store_id_valid store_store_commute)   
+      using assms prefix_contains_msg by (metis concurrent_store_store_independent store_id_valid store_store_commute)   
   } thus ?thesis
     by(fastforce simp: hb.concurrent_ops_commute_def)
 qed
 
 theorem (in imap) convergence:
   assumes "set (node_deliver_messages xs) = set (node_deliver_messages ys)"
-      and "xs prefix of i" and "ys prefix of j"
-    shows "apply_operations xs = apply_operations ys"
+    and "xs prefix of i" 
+    and "ys prefix of j"
+  shows "apply_operations xs = apply_operations ys"
 using assms by(auto simp add: apply_operations_def intro: hb.convergence_ext concurrent_operations_commute
                 node_deliver_messages_distinct hb_consistent_prefix)
               
